AAC_tactics, version 0.2-pl2 dans branches/v8.3
git-svn-id: svn://scm.gforge.inria.fr/svnroot/coq-contribs/branches/v8.3@1350 0cf17b13-060f-0410-b1b1-c666bec9822a

AAC_coq.ml
@@ -1,0 +1,591 @@
+(***************************************************************************)
+(*  This is part of aac_tactics, it is distributed under the terms of the  *)
+(*         GNU Lesser General Public License version 3                     *)
+(*              (see file LICENSE for more details)                        *)
+(*                                                                         *)
+(*       Copyright 2009-2010: Thomas Braibant, Damien Pous.                *)
+(***************************************************************************)
+
+(** Interface with Coq *)
+type constr = Term.constr
+
+open Term
+open Names
+open Coqlib
+
+(* The contrib name is used to locate errors when loading constrs *)
+let contrib_name = "aac_tactics"
+
+(* Getting constrs (primitive Coq terms) from existing Coq
+   libraries. *)
+let find_constant contrib dir s =
+  Libnames.constr_of_global (Coqlib.find_reference contrib dir s)
+
+let init_constant dir s = find_constant contrib_name dir s
+
+(* A clause specifying that the [let] should not try to fold anything
+   in the goal *)
+let nowhere =
+  { Tacexpr.onhyps = Some [];
+    Tacexpr.concl_occs = Rawterm.no_occurrences_expr
+  }
+
+let cps_mk_letin
+    (name:string)
+    (c: constr)
+    (k : constr -> Proof_type.tactic)
+: Proof_type.tactic =
+  fun goal ->
+    let name = (Names.id_of_string name) in
+    let name =  Tactics.fresh_id [] name goal in
+    let letin = (Tactics.letin_tac None  (Name name) c None nowhere) in
+      Tacticals.tclTHEN letin (k (mkVar name)) goal
+
+(** {2 General functions}  *)
+
+type goal_sigma =  Proof_type.goal Tacmach.sigma
+let goal_update (goal : goal_sigma) evar_map : goal_sigma=
+  let it = Tacmach.sig_it goal in
+    Tacmach.re_sig it evar_map
+
+let fresh_evar goal ty : constr * goal_sigma =
+  let env = Tacmach.pf_env goal in
+  let evar_map = Tacmach.project goal in
+  let (em,x) = Evarutil.new_evar evar_map env ty in
+    x,( goal_update goal em)
+     
+let resolve_one_typeclass goal ty : constr*goal_sigma=
+  let env = Tacmach.pf_env goal in
+  let evar_map = Tacmach.project goal in
+  let em,c = Typeclasses.resolve_one_typeclass env evar_map ty in
+    c, (goal_update goal em)
+
+let general_error =
+  "Cannot resolve a typeclass : please report"
+
+let cps_resolve_one_typeclass ?error : Term.types -> (Term.constr  -> Proof_type.tactic) -> Proof_type.tactic = fun t k  goal  ->
+  Tacmach.pf_apply
+    (fun env em -> let em ,c =  
+		  try Typeclasses.resolve_one_typeclass env em t
+		  with Not_found ->
+		    begin match error with
+		      | None -> Util.anomaly  "Cannot resolve a typeclass : please report"
+		      | Some x -> Util.error x
+		    end
+		in
+		Tacticals.tclTHENLIST [Refiner.tclEVARS em; k c] goal
+    )	goal
+
+
+let nf_evar goal c : Term.constr=
+  let evar_map = Tacmach.project goal in
+    Evarutil.nf_evar evar_map c
+
+let evar_unit (gl : goal_sigma) (x : constr) : constr * goal_sigma =
+  let env = Tacmach.pf_env gl in
+  let evar_map = Tacmach.project gl in
+  let (em,x) = Evarutil.new_evar evar_map env x in
+    x,(goal_update gl em)
+     
+let evar_binary (gl: goal_sigma) (x : constr) =
+  let env = Tacmach.pf_env gl in
+  let evar_map = Tacmach.project gl in
+  let ty = mkArrow x (mkArrow x x) in
+  let (em,x) = Evarutil.new_evar evar_map env  ty in
+    x,( goal_update gl em)
+
+let evar_relation (gl: goal_sigma) (x: constr) =
+  let env = Tacmach.pf_env gl in
+  let evar_map = Tacmach.project gl in
+  let ty = mkArrow x (mkArrow x (mkSort prop_sort)) in
+  let (em,r) = Evarutil.new_evar evar_map env  ty in
+    r,( goal_update gl em)
+
+let cps_evar_relation (x: constr) k = fun goal -> 
+  Tacmach.pf_apply
+    (fun env em ->
+      let ty = mkArrow x (mkArrow x (mkSort prop_sort)) in
+      let (em,r) = Evarutil.new_evar em env  ty in 	
+      Tacticals.tclTHENLIST [Refiner.tclEVARS em; k r] goal
+    )	goal
+
+(* decomp_term :  constr -> (constr, types) kind_of_term *)
+let decomp_term c = kind_of_term (strip_outer_cast c)
+   
+let lapp c v  = mkApp (Lazy.force c, v)
+
+(** {2 Bindings with Coq' Standard Library}  *)
+module Std = struct  		
+(* Here we package the module to be able to use List, later *)
+
+module Pair = struct
+ 
+  let path = ["Coq"; "Init"; "Datatypes"]
+  let typ = lazy (init_constant path "prod")
+  let pair = lazy (init_constant path "pair")
+  let of_pair t1 t2 (x,y) =
+    mkApp (Lazy.force pair,  [| t1; t2; x ; y|] )
+end
+
+module Bool = struct
+  let path = ["Coq"; "Init"; "Datatypes"]
+  let typ = lazy (init_constant path "bool")
+  let ctrue = lazy (init_constant path "true")
+  let cfalse = lazy (init_constant path "false")
+  let of_bool  b =
+    if b then Lazy.force ctrue else Lazy.force cfalse
+end
+
+module Comparison = struct
+  let path = ["Coq"; "Init"; "Datatypes"]
+  let typ = lazy (init_constant path "comparison")
+  let eq = lazy (init_constant path "Eq")
+  let lt = lazy (init_constant path "Lt")
+  let gt = lazy (init_constant path "Gt")
+end
+
+module Leibniz = struct
+  let path = ["Coq"; "Init"; "Logic"]
+  let eq_refl = lazy (init_constant path "eq_refl")
+  let eq_refl ty x = lapp eq_refl [| ty;x|]
+end
+
+module Option = struct
+  let path = ["Coq"; "Init"; "Datatypes"]
+  let typ = lazy (init_constant path "option")
+  let some = lazy (init_constant path "Some")
+  let none = lazy (init_constant path "None")
+  let some t x = mkApp (Lazy.force some, [| t ; x|])
+  let none t = mkApp (Lazy.force none, [| t |])
+  let of_option t x = match x with
+    | Some x -> some t x
+    | None -> none t
+end   
+
+module Pos = struct
+   
+    let path = ["Coq" ; "NArith"; "BinPos"]
+    let typ = lazy (init_constant path "positive")
+    let xI =      lazy (init_constant path "xI")
+    let xO =      lazy (init_constant path "xO")
+    let xH =      lazy (init_constant path "xH")
+
+    (* A coq positive from an int *)
+    let of_int n =
+      let rec aux n =
+	begin  match n with
+	  | n when n < 1 -> assert false
+	  | 1 -> Lazy.force xH
+	  | n -> mkApp
+	      (
+		(if n mod 2 = 0
+		 then Lazy.force xO
+		 else Lazy.force xI
+		),  [| aux (n/2)|]
+	      )
+	end
+      in
+	aux n
+end
+   
+module Nat = struct
+  let path = ["Coq" ; "Init"; "Datatypes"]
+  let typ = lazy (init_constant path "nat")
+  let _S =      lazy (init_constant  path "S")
+  let _O =      lazy (init_constant  path "O")
+    (* A coq nat from an int *)
+  let of_int n =
+    let rec aux n =
+      begin  match n with
+	| n when n < 0 -> assert false
+	| 0 -> Lazy.force _O
+	| n -> mkApp
+	    (
+	      (Lazy.force _S
+	      ),  [| aux (n-1)|]
+	    )
+      end
+    in
+      aux n
+end
+   
+(** Lists from the standard library*)
+module List = struct
+  let path = ["Coq"; "Lists"; "List"]
+  let typ = lazy (init_constant path "list")
+  let nil = lazy (init_constant path "nil")
+  let cons = lazy (init_constant path "cons")
+  let cons ty h t =
+    mkApp (Lazy.force cons, [|  ty; h ; t |])
+  let nil ty =
+    (mkApp (Lazy.force nil, [|  ty |]))
+  let rec of_list ty = function
+    | [] -> nil ty
+    | t::q -> cons ty t (of_list  ty q)
+  let type_of_list ty =
+    mkApp (Lazy.force typ, [|ty|])
+end
+   
+(** Morphisms *)
+module Classes =
+struct
+  let classes_path = ["Coq";"Classes"; ]
+  let morphism = lazy (init_constant (classes_path@["Morphisms"]) "Proper")
+  let equivalence = lazy (init_constant (classes_path@ ["RelationClasses"]) "Equivalence")
+  let reflexive = lazy (init_constant (classes_path@ ["RelationClasses"]) "Reflexive")
+  let transitive = lazy (init_constant (classes_path@ ["RelationClasses"]) "Transitive")
+
+  (** build the type [Equivalence ty rel]  *)
+  let mk_equivalence ty rel =
+    mkApp (Lazy.force equivalence, [| ty; rel|])
+
+
+  (** build the type [Reflexive ty rel]  *)
+  let mk_reflexive ty rel =
+    mkApp (Lazy.force reflexive, [| ty; rel|])
+
+  (** build the type [Proper rel t] *)
+  let mk_morphism ty rel t =
+    mkApp (Lazy.force morphism, [| ty; rel; t|])
+
+  (** build the type [Transitive ty rel]  *)
+  let mk_transitive ty rel =
+    mkApp (Lazy.force transitive, [| ty; rel|])
+end
+
+module Relation = struct
+  type t =
+      {
+	carrier : constr;
+	r : constr;
+      }
+	
+  let make ty r = {carrier = ty; r = r }
+  let split t = t.carrier, t.r
+end
+   
+module Transitive = struct
+  type t =
+      {
+	carrier : constr;
+	leq : constr;
+	transitive : constr;
+      }
+  let make ty leq transitive = {carrier = ty; leq = leq; transitive = transitive}
+  let infer goal ty leq  =
+    let ask = Classes.mk_transitive ty leq in
+    let transitive , goal = resolve_one_typeclass goal ask in
+      make ty leq transitive, goal
+  let from_relation goal rlt =
+    infer goal (rlt.Relation.carrier) (rlt.Relation.r)
+  let cps_from_relation rlt k =
+    let ty =rlt.Relation.carrier in
+    let r = rlt.Relation.r in
+    let ask = Classes.mk_transitive  ty r in
+    cps_resolve_one_typeclass ask
+      (fun trans -> k (make ty r trans) )
+  let to_relation t =
+    {Relation.carrier = t.carrier; Relation.r = t.leq}
+
+end
+	
+module Equivalence = struct
+  type t =
+      {
+	carrier : constr;
+	eq : constr;
+	equivalence : constr;	
+      }
+  let make ty eq equivalence = {carrier = ty; eq = eq; equivalence = equivalence}
+  let infer goal ty eq  =
+    let ask = Classes.mk_equivalence ty eq in
+    let equivalence , goal = resolve_one_typeclass goal ask in
+      make ty eq equivalence, goal 	 
+  let from_relation goal rlt =
+    infer goal (rlt.Relation.carrier) (rlt.Relation.r)
+  let cps_from_relation rlt k =
+    let ty =rlt.Relation.carrier in
+    let r = rlt.Relation.r in
+    let ask = Classes.mk_equivalence  ty r in
+    cps_resolve_one_typeclass ask (fun equiv -> k (make ty r equiv) )
+  let to_relation t =
+    {Relation.carrier = t.carrier; Relation.r = t.eq}
+  let split t =
+    t.carrier, t.eq, t.equivalence
+end
+end
+(**[ match_as_equation goal eqt] see [eqt] as an equation. An
+   optionnal rel_context can be provided to ensure taht the term
+   remains typable*)
+let match_as_equation ?(context = Term.empty_rel_context) goal equation : (constr*constr* Std.Relation.t) option  =
+  let env = Tacmach.pf_env goal in
+  let env =  Environ.push_rel_context context env in
+  let evar_map = Tacmach.project goal in
+  begin
+    match decomp_term equation with
+      | App(c,ca) when Array.length ca >= 2 ->
+	let n = Array.length ca  in
+	let left  =  ca.(n-2) in
+	let right =  ca.(n-1) in
+	let r = (mkApp (c, Array.sub ca 0 (n - 2))) in
+	let carrier =  Typing.type_of env evar_map left in
+	let rlt =Std.Relation.make carrier r
+	in
+	Some (left, right, rlt )
+      | _ -> None
+  end
+
+
+(** {1 Tacticals}  *)
+
+let tclTIME msg tac = fun gl ->
+  let u = Sys.time () in
+  let r = tac gl in
+  let _ = Pp.msgnl (Pp.str (Printf.sprintf "%s:%fs" msg (Sys.time ()-.  u))) in
+    r
+
+let tclDEBUG msg tac = fun gl ->
+  let _ = Pp.msgnl (Pp.str msg) in
+    tac gl
+
+let tclPRINT  tac = fun gl ->
+  let _ = Pp.msgnl (Printer.pr_constr (Tacmach.pf_concl gl)) in
+    tac gl
+
+
+(** {1 Error related mechanisms}  *)
+(* functions to handle the failures of our tactic. Some should be
+   reported [anomaly], some are on behalf of the user [user_error]*)
+let anomaly msg =
+  Util.anomaly ("[aac_tactics] " ^ msg)
+
+let user_error msg =
+  Util.error ("[aac_tactics] " ^ msg)
+
+let warning msg =
+  Pp.msg_warning (Pp.str ("[aac_tactics]" ^ msg))
+
+     
+(** {1 Rewriting tactics used in aac_rewrite}  *)
+module Rewrite = struct
+(** Some informations about the hypothesis, with an (informal)
+    invariant:
+    - [typeof hyp = hyptype]
+    - [hyptype = forall context, body]
+    - [body = rel left right]
+ 
+*)
+
+type hypinfo =
+    {
+      hyp : Term.constr;		  (** the actual constr corresponding to the hypothese  *)
+      hyptype : Term.constr; 		(** the type of the hypothesis *)
+      context : Term.rel_context; 	(** the quantifications of the hypothese *)
+      body : Term.constr; 		(** the body of the type of the hypothesis*)
+      rel : Std.Relation.t; 		(** the relation  *)
+      left : Term.constr;		(** left hand side *)
+      right : Term.constr;		(** right hand side  *)
+      l2r : bool; 			(** rewriting from left to right  *)
+    }
+
+let get_hypinfo c ~l2r ?check_type  (k : hypinfo -> Proof_type.tactic) :    Proof_type.tactic = fun goal ->
+  let ctype =  Tacmach.pf_type_of goal c in 
+  let (rel_context, body_type) = Term.decompose_prod_assum ctype in 
+  let rec check f e =
+    match decomp_term e with
+      | Term.Rel i ->
+	    let name, constr_option, types = Term.lookup_rel i rel_context
+	    in f types
+      | _ -> Term.fold_constr (fun acc x -> acc && check f x) true e
+  in
+  begin match check_type with
+    | None -> ()
+    | Some f ->
+      if not (check f body_type)
+      then user_error "Unable to deal with higher-order or heterogeneous patterns";
+  end;
+  begin
+    match match_as_equation ~context:rel_context  goal body_type with
+      | None -> 
+	user_error "The hypothesis is not an applied relation"
+      |  Some (hleft,hright,hrlt) ->
+	k {
+    	  hyp = c;
+    	  hyptype = ctype;
+	  body =  body_type;
+	  l2r = l2r;
+    	  context = rel_context;
+    	  rel = hrlt ;
+    	  left =hleft;
+    	  right = hright;
+	}
+	goal
+  end
+   
+
+(* The problem : Given a term to rewrite of type [H :forall xn ... x1,
+   t], we have to instanciate the subset of [xi] of type
+   [carrier]. [subst : (int * constr)] is the mapping the debruijn
+   indices in [t] to the [constrs]. We need to handle the rest of the
+   indexes. Two ways :
+
+   - either using fresh evars and rewriting [H tn ?1 tn-2 ?2 ]
+   - either building a term like [fun 1 2 => H tn 1 tn-2 2]
+
+   Both these terms have the same type.
+*)
+
+
+(* Fresh evars for everyone (should be the good way to do this
+   recompose in Coq v8.4) *)
+let recompose_prod 
+    (context : Term.rel_context)
+    (subst : (int * Term.constr) list)
+    env
+    em
+    : Evd.evar_map * Term.constr list =
+  (* the last index of rel relevant for the rewriting *)
+  let min_n = List.fold_left
+    (fun acc (x,_) -> min acc x)
+    (List.length context) subst in 
+  let rec aux context acc em n =
+    let _ = Printf.printf "%i\n%!" n in
+    match context with
+      | [] ->
+	env, em, acc
+      | ((name,c,ty) as t)::q ->
+	let env, em, acc = aux q acc em (n+1) in
+	if n >= min_n
+	then
+	  let em,x =
+	    try em, List.assoc n subst
+	    with | Not_found ->
+	      Evarutil.new_evar em env (Term.substl acc ty)
+	  in
+	  (Environ.push_rel t env), em,x::acc
+	else
+	  env,em,acc
+  in
+  let _,em,acc = aux context [] em 1 in
+  em, acc
+
+(* no fresh evars : instead, use a lambda abstraction around an
+   application to handle non-instanciated variables. *)
+   
+let recompose_prod'
+    (context : Term.rel_context)
+    (subst : (int *Term.constr) list)
+    c
+    =
+  let rec popn pop n l =
+    if n <= 0 then l
+    else match l with
+      | [] -> []
+      | t::q -> pop t :: (popn pop (n-1) q)
+  in
+  let pop_rel_decl (name,c,ty) = (name,c,Termops.pop ty) in
+  let rec aux sign n next app ctxt =
+    match sign with
+      | [] -> List.rev app, List.rev ctxt
+      | decl::sign ->
+	try let term =  (List.assoc n subst) in
+	    aux sign (n+1) next (term::app) (None :: ctxt)
+	with
+	  | Not_found ->
+	    let term = Term.mkRel next in
+	    aux sign (n+1) (next+1) (term::app) (Some decl :: ctxt)
+  in
+  let app,ctxt = aux context 1 1 [] [] in
+  (* substitutes in the context *)
+  let rec update ctxt app =
+    match ctxt,app with
+      | [],_ -> []
+      | _,[] -> []
+      | None :: sign, _ :: app ->
+	None ::	update sign (List.map (Termops.pop) app)
+      | Some decl :: sign, _ :: app ->
+	Some (Term.substl_decl app decl)::update sign (List.map (Termops.pop) app) 
+  in
+  let ctxt = update ctxt app in
+  (* updates the rel accordingly, taking some care not to go to far
+     beyond: it is important not to lift indexes homogeneously, we
+     have to update *)
+  let rec update ctxt res n =
+    match ctxt with
+      | [] -> List.rev res
+      | None :: sign ->
+  	(update (sign) (popn pop_rel_decl n res) 0)
+      | Some decl :: sign ->
+  	update sign (decl :: res) (n+1)
+  in
+  let ctxt = update ctxt [] 0 in
+  let c = Term.applistc c (List.rev app) in
+  let c = Term.it_mkLambda_or_LetIn c (ctxt) in
+  c
+
+(* Version de Matthieu
+let subst_rel_context k cstr ctx =
+  let (_, ctx') =
+    List.fold_left (fun (k, ctx') (id, b, t) -> (succ k, (id, Option.map
+      (Term.substnl [cstr] k) b, Term.substnl [cstr] k t) :: ctx')) (k, [])
+      ctx in List.rev ctx'
+
+let recompose_prod' context subst c =
+  let len = List.length context in
+  let rec aux sign n next app ctxt =
+    match sign with
+    | [] -> List.rev app, List.rev ctxt
+    | decl::sign ->
+	try let term = (List.assoc n subst) in
+	  aux (subst_rel_context 0 term sign) (pred n) (succ next)
+	    (term::List.map (Term.lift (-1)) app) ctxt
+	with Not_found ->
+	  let term = Term.mkRel (len - next) in
+	    aux sign (pred n) (succ next) (term::app) (decl :: ctxt)
+  in
+  let app,ctxt = aux (List.rev context) len 0 [] [] in
+    Term.it_mkLambda_or_LetIn (Term.applistc c(app)) (List.rev ctxt)
+*)
+
+let build
+    (h : hypinfo)
+    (subst : (int *Term.constr) list)
+    (k :Term.constr -> Proof_type.tactic)
+    : Proof_type.tactic = fun goal ->
+      let c = recompose_prod' h.context subst h.hyp in
+      Tacticals.tclTHENLIST [k c] goal
+
+let build_with_evar
+    (h : hypinfo)
+    (subst : (int *Term.constr) list)
+    (k :Term.constr -> Proof_type.tactic)
+    : Proof_type.tactic
+    = fun goal ->
+      Tacmach.pf_apply
+	(fun env em ->
+	  let evar_map,  acc = recompose_prod h.context subst env em in
+	  let c = Term.applistc h.hyp (List.rev acc) in
+	  Tacticals.tclTHENLIST [Refiner.tclEVARS evar_map; k c] goal
+	) goal
+
+
+let rewrite ?(abort=false)hypinfo subst k =
+  build hypinfo subst
+    (fun rew ->
+      let tac =
+	if not abort then
+	  Equality.general_rewrite_bindings
+	    hypinfo.l2r
+	    Termops.all_occurrences
+	    false
+	    (rew,Rawterm.NoBindings)
+	    true
+	else
+	  Tacticals.tclIDTAC
+      in k tac
+    )
+
+
+end
+
+include Std
