AAC_rewrite.ml
@@ -1,0 +1,524 @@
+(***************************************************************************)
+(*  This is part of aac_tactics, it is distributed under the terms of the  *)
+(*         GNU Lesser General Public License version 3                     *)
+(*              (see file LICENSE for more details)                        *)
+(*                                                                         *)
+(*       Copyright 2009-2010: Thomas Braibant, Damien Pous.                *)
+(***************************************************************************)
+
+(** aac_rewrite -- rewriting modulo  *)
+
+
+module Control =   struct
+    let debug = false
+    let printing = false
+    let time = false
+end
+
+module Debug = AAC_helper.Debug (Control)
+open Debug
+
+let time_tac msg tac =
+  if Control.time then  AAC_coq.tclTIME msg tac else tac
+
+let tac_or_exn tac exn msg = fun gl ->
+  try tac gl with e ->
+    pr_constr "last goal" (Tacmach.pf_concl gl);
+    exn msg e
+
+(* helper to be used with the previous function: raise a new anomaly
+   except if a another one was previously raised *)
+let push_anomaly msg = function
+  | Util.Anomaly _ as e -> raise e
+  | _ -> AAC_coq.anomaly msg
+
+module M = AAC_matcher
+
+open Term
+open Names
+open Coqlib
+open Proof_type
+
+(** The various kind of relation we can encounter, as a hierarchy *)
+type rew_relation =
+  | Bare of AAC_coq.Relation.t
+  | Transitive of AAC_coq.Transitive.t
+  | Equivalence of AAC_coq.Equivalence.t
+
+(** {!promote try to go higher in the aforementionned hierarchy} *)
+let promote (rlt : AAC_coq.Relation.t) (k : rew_relation -> Proof_type.tactic) =
+  try AAC_coq.Equivalence.cps_from_relation rlt
+	(fun e -> k (Equivalence e))
+  with
+    | Not_found ->
+      begin
+	try AAC_coq.Transitive.cps_from_relation rlt
+	      (fun trans -> k (Transitive trans))
+	with
+	  |Not_found -> k (Bare rlt)
+      end
+
+
+(*
+  Various situations:
+  p == q |- left == right : rewrite <- ->
+  p <= q |- left <= right : rewrite ->
+  p <= q |- left == right : failure
+  p == q |- left <= right : rewrite <- ->
+ 
+  Not handled
+  p <= q |- left >= right : failure
+*)
+
+(** aac_lift : the ideal type beyond AAC.v/AAC_lift
+
+    A base relation r, together with an equivalence relation, and the
+    proof that the former lifts to the later. Howver, we have to
+    ensure manually the invariant : r.carrier == e.carrier, and that
+    lift connects the two things *)
+type aac_lift =
+    {
+      r : AAC_coq.Relation.t;
+      e : AAC_coq.Equivalence.t;
+      lift : Term.constr    
+    }
+     
+type rewinfo =
+    {
+      hypinfo : AAC_coq.Rewrite.hypinfo;
+     
+      in_left : bool; 	     		(** are we rewriting in the left hand-sie of the goal *)
+      pattern : constr;
+      subject : constr;
+      morph_rlt : AAC_coq.Relation.t; (** the relation we look for in morphism *)
+      eqt : AAC_coq.Equivalence.t;    (** the equivalence we use as workbase *)
+      rlt : AAC_coq.Relation.t;	  (** the relation in the goal  *)
+      lifting: aac_lift
+    }
+
+let infer_lifting (rlt: AAC_coq.Relation.t) (k : lift:aac_lift -> Proof_type.tactic) : Proof_type.tactic =
+  AAC_coq.cps_evar_relation rlt.AAC_coq.Relation.carrier (fun e ->
+    let lift_ty =
+      mkApp (Lazy.force AAC_theory.Stubs.lift,
+	     [|
+	       rlt.AAC_coq.Relation.carrier;
+	       rlt.AAC_coq.Relation.r;
+	       e
+	     |]
+      ) in
+    AAC_coq.cps_resolve_one_typeclass ~error:"Cannot infer a lifting"
+      lift_ty (fun lift goal ->
+      let x = rlt.AAC_coq.Relation.carrier in
+      let r = rlt.AAC_coq.Relation.r in
+      let eq =  (AAC_coq.nf_evar goal e) in 
+      let equiv = AAC_coq.lapp AAC_theory.Stubs.lift_proj_equivalence [| x;r;eq; lift |] in
+      let lift =
+	{
+	  r = rlt;
+	  e = AAC_coq.Equivalence.make x eq equiv;
+	  lift = lift;
+	}
+      in
+      k ~lift:lift  goal
+    ))
+     
+(** Builds a rewinfo, once and for all *)
+let dispatch in_left (left,right,rlt) hypinfo (k: rewinfo -> Proof_type.tactic ) : Proof_type.tactic=
+  let l2r = hypinfo.AAC_coq.Rewrite.l2r in
+  infer_lifting rlt
+    (fun ~lift ->
+      let eq = lift.e in
+      k {
+	hypinfo = hypinfo;
+	in_left = in_left;
+	pattern = if l2r then hypinfo.AAC_coq.Rewrite.left else hypinfo.AAC_coq.Rewrite.right;
+	subject = if in_left then  left else right;
+	morph_rlt = AAC_coq.Equivalence.to_relation eq;
+	eqt = eq;
+	lifting = lift;
+	rlt = rlt
+      }
+    )
+   
+   
+
+(** {1 Tactics} *)
+
+
+(** Build the reifiers, the reified terms, and the evaluation fonction  *)
+let handle eqt zero envs (t : AAC_matcher.Terms.t) (t' : AAC_matcher.Terms.t) k =
+
+  let (x,r,_) = AAC_coq.Equivalence.split eqt  in
+  AAC_theory.Trans.mk_reifier (AAC_coq.Equivalence.to_relation eqt) zero envs 
+    (fun (maps, reifier) ->
+      (* fold through a term and reify *)
+      let t = AAC_theory.Trans.reif_constr_of_t reifier t in
+      let t' = AAC_theory.Trans.reif_constr_of_t reifier  t' in
+      (* Some letins  *)
+      let eval = (mkApp (Lazy.force AAC_theory.Stubs.eval, [|x;r; maps.AAC_theory.Trans.env_sym; maps.AAC_theory.Trans.env_bin; maps.AAC_theory.Trans.env_units|])) in
+     
+      AAC_coq.cps_mk_letin "eval" eval (fun eval ->
+	AAC_coq.cps_mk_letin "left" t (fun t ->
+	  AAC_coq.cps_mk_letin "right" t' (fun t' ->
+	    k maps eval t t'))))
+
+(** [by_aac_reflexivity] is a sub-tactic that closes a sub-goal that
+      is merely a proof of equality of two terms modulo AAC *) 
+let by_aac_reflexivity zero
+    eqt envs (t : AAC_matcher.Terms.t) (t' : AAC_matcher.Terms.t) : Proof_type.tactic =
+  handle eqt zero envs t t'
+    (fun maps eval t t' ->
+      let (x,r,e) = AAC_coq.Equivalence.split eqt in
+      let decision_thm = AAC_coq.lapp AAC_theory.Stubs.decide_thm
+	[|x;r;e;
+	  maps.AAC_theory.Trans.env_sym;
+	  maps.AAC_theory.Trans.env_bin;
+	  maps.AAC_theory.Trans.env_units;
+	  t;t';
+	|]
+      in
+      (* This convert is required to deal with evars in a proper
+	 way *)
+      let convert_to = mkApp (r, [| mkApp (eval,[| t |]); mkApp (eval, [|t'|])|])   in
+      let convert = Tactics.convert_concl convert_to Term.VMcast in
+      let apply_tac = Tactics.apply decision_thm in
+      (Tacticals.tclTHENLIST
+	 [
+	   convert ;
+	   tac_or_exn apply_tac AAC_coq.user_error "unification failure";
+	   tac_or_exn (time_tac "vm_norm" (Tactics.normalise_in_concl)) AAC_coq.anomaly "vm_compute failure";
+	   Tacticals.tclORELSE Tactics.reflexivity
+	     (Tacticals.tclFAIL 0 (Pp.str "Not an equality modulo A/AC"))
+	 ])
+    )
+
+let by_aac_normalise zero lift ir t t' =
+  let eqt = lift.e in
+  let rlt = lift.r in
+  handle eqt zero ir t t'
+    (fun  maps eval t t' ->
+      let (x,r,e) = AAC_coq.Equivalence.split eqt in
+      let normalise_thm = AAC_coq.lapp AAC_theory.Stubs.lift_normalise_thm
+	[|x;r;e;
+	  maps.AAC_theory.Trans.env_sym;
+	  maps.AAC_theory.Trans.env_bin;
+	  maps.AAC_theory.Trans.env_units;
+	  rlt.AAC_coq.Relation.r;
+	  lift.lift;
+	  t;t';
+	|]
+      in
+      (* This convert is required to deal with evars in a proper
+	 way *)
+      let convert_to = mkApp (rlt.AAC_coq.Relation.r, [| mkApp (eval,[| t |]); mkApp (eval, [|t'|])|])   in
+      let convert = Tactics.convert_concl convert_to Term.VMcast in
+      let apply_tac = Tactics.apply normalise_thm in
+      (Tacticals.tclTHENLIST
+	 [
+	   convert ;
+	   apply_tac;
+	 ])
+	
+    )
+
+(** A handler tactic, that reifies the goal, and infer the liftings,
+    and then call its continuation *)
+let aac_conclude
+    (k : Term.constr -> aac_lift -> AAC_theory.Trans.ir -> AAC_matcher.Terms.t -> AAC_matcher.Terms.t -> Proof_type.tactic) = fun goal ->
+
+    let (equation : Term.types) = Tacmach.pf_concl goal in
+    let envs = AAC_theory.Trans.empty_envs () in
+    let left, right,r =
+      match AAC_coq.match_as_equation goal equation with
+	| None -> AAC_coq.user_error "The goal is not an applied relation"
+	| Some x -> x in    
+    try infer_lifting r
+      (fun ~lift  goal ->
+	let eq = AAC_coq.Equivalence.to_relation lift.e in
+	let tleft,tright, goal = AAC_theory.Trans.t_of_constr goal eq envs (left,right)   in
+	let goal, ir = AAC_theory.Trans.ir_of_envs goal eq envs in
+	let concl = Tacmach.pf_concl goal in
+	let _ = pr_constr "concl "concl in 	     
+	let evar_map = Tacmach.project goal in
+	Tacticals.tclTHEN
+	  (Refiner.tclEVARS evar_map)
+	  (k left lift ir tleft tright)
+	  goal
+      )goal
+  with
+    | Not_found -> AAC_coq.user_error "No lifting from the goal's relation to an equivalence"
+
+open Libnames
+open Tacinterp
+
+let aac_normalise = fun goal ->
+  let ids = Tacmach.pf_ids_of_hyps goal in
+  Tacticals.tclTHENLIST
+    [
+      aac_conclude by_aac_normalise;
+      Tacinterp.interp (
+      	<:tactic<
+	  intro x;
+	  intro y;
+	  vm_compute in x;
+	  vm_compute in y;
+	  unfold x;
+	  unfold y;
+      	  compute [Internal.eval Internal.fold_map Internal.copy Prect]; simpl
+      	>>
+      );
+      Tactics.keep ids
+    ] goal
+
+let aac_reflexivity = fun goal ->
+  aac_conclude
+    (fun zero lift ir t t' ->
+      let x,r = AAC_coq.Relation.split (lift.r) in
+      let r_reflexive = (AAC_coq.Classes.mk_reflexive x r) in
+      AAC_coq.cps_resolve_one_typeclass ~error:"The goal's relation is not reflexive"
+	r_reflexive
+	(fun reflexive ->
+	  let lift_reflexivity =
+	    mkApp (Lazy.force (AAC_theory.Stubs.lift_reflexivity),
+		   [|
+		     x;
+		     r;
+		     lift.e.AAC_coq.Equivalence.eq;
+		     lift.lift;
+		     reflexive
+		   |])
+	  in
+	  Tacticals.tclTHEN
+	    (Tactics.apply lift_reflexivity)
+	    (fun goal ->
+	      let concl = Tacmach.pf_concl goal in
+	      let _ = pr_constr "concl "concl in 	     
+	      by_aac_reflexivity zero lift.e ir t t' goal)
+	)
+    ) goal
+
+(** A sub-tactic to lift the rewriting using AAC_lift  *)
+let lift_transitivity in_left (step:constr) preorder lifting (using_eq : AAC_coq.Equivalence.t): tactic =
+  fun goal ->
+    (* catch the equation and the two members*)
+    let concl = Tacmach.pf_concl goal in
+    let (left, right, _ ) = match  AAC_coq.match_as_equation goal concl with
+      | Some x -> x
+      | None -> AAC_coq.user_error "The goal is not an equation"
+    in
+    let lift_transitivity =
+      let thm = 
+	if in_left
+	then
+	  Lazy.force AAC_theory.Stubs.lift_transitivity_left
+	else
+	  Lazy.force AAC_theory.Stubs.lift_transitivity_right
+      in
+      mkApp (thm,
+	     [|
+	       preorder.AAC_coq.Relation.carrier;
+	       preorder.AAC_coq.Relation.r;
+	       using_eq.AAC_coq.Equivalence.eq;
+	       lifting;
+	       step;
+	       left;
+	       right;
+	     |])
+    in
+    Tacticals.tclTHENLIST
+      [
+	Tactics.apply lift_transitivity
+      ] goal
+
+
+(** The core tactic for aac_rewrite *)
+let core_aac_rewrite ?abort
+    rewinfo
+    subst
+    (by_aac_reflexivity : AAC_matcher.Terms.t -> AAC_matcher.Terms.t -> Proof_type.tactic)
+    (tr : constr) t left : tactic =
+  pr_constr "transitivity through" tr;   
+  let tran_tac =
+    lift_transitivity rewinfo.in_left tr rewinfo.rlt rewinfo.lifting.lift rewinfo.eqt
+  in
+  AAC_coq.Rewrite.rewrite ?abort rewinfo.hypinfo subst (fun rew -> 
+    Tacticals.tclTHENSV
+      (tac_or_exn (tran_tac) AAC_coq.anomaly "Unable to make the transitivity step")
+      (
+	if rewinfo.in_left
+	then [| by_aac_reflexivity left t ; rew |]
+	else [| by_aac_reflexivity t left ; rew  |]
+      )
+  )
+
+exception NoSolutions
+
+
+(** Choose a substitution from a
+    [(int * Terms.t * Env.env AAC_search_monad.m) AAC_search_monad.m ] *)
+(* WARNING: Beware, since the printing function can change the order of the
+   printed monad, this function has to be updated accordingly *)
+let choose_subst  subterm sol m=
+  try
+    let (depth,pat,envm) =  match subterm with
+      | None -> 			(* first solution *)
+	List.nth ( List.rev (AAC_search_monad.to_list m)) 0
+      | Some x ->
+	List.nth ( List.rev (AAC_search_monad.to_list m)) x
+    in
+    let env = match sol with
+	None -> 	
+	  List.nth ( (AAC_search_monad.to_list envm)) 0
+      | Some x ->  List.nth ( (AAC_search_monad.to_list envm)) x
+    in
+    pat, env
+  with
+    | _ -> raise NoSolutions
+	
+(** rewrite the constr modulo AC from left to right in the left member
+    of the goal *)
+let aac_rewrite  ?abort rew ?(l2r=true) ?(show = false) ?(in_left=true) ?strict ~occ_subterm ~occ_sol ?extra : Proof_type.tactic  = fun goal ->
+  let envs = AAC_theory.Trans.empty_envs () in
+  let (concl : Term.types) = Tacmach.pf_concl goal in
+  let (_,_,rlt) as concl =
+    match AAC_coq.match_as_equation goal concl with
+      | None -> AAC_coq.user_error "The goal is not an applied relation"
+      | Some (left, right, rlt) -> left,right,rlt
+  in
+  let check_type x =
+    Tacmach.pf_conv_x goal x rlt.AAC_coq.Relation.carrier
+  in
+  AAC_coq.Rewrite.get_hypinfo rew ~l2r ?check_type:(Some check_type)
+    (fun hypinfo ->
+      dispatch in_left concl hypinfo
+	(	
+	  fun rewinfo ->
+	    let goal =
+	      match extra with
+		| Some t -> AAC_theory.Trans.add_symbol goal rewinfo.morph_rlt envs t
+		| None -> goal
+	    in
+	    let pattern, subject, goal =
+	      AAC_theory.Trans.t_of_constr goal rewinfo.morph_rlt envs
+		(rewinfo.pattern , rewinfo.subject)  
+	    in
+	    let goal, ir = AAC_theory.Trans.ir_of_envs goal rewinfo.morph_rlt envs in
+
+	    let units = AAC_theory.Trans.ir_to_units ir in
+	    let m =  AAC_matcher.subterm ?strict units pattern subject in
+	    (* We sort the monad in increasing size of contet *)
+	    let m = AAC_search_monad.sort (fun (x,_,_) (y,_,_) -> x -  y) m in
+	   
+	    if show
+	    then	      
+	      AAC_print.print rewinfo.morph_rlt ir m (hypinfo.AAC_coq.Rewrite.context) 
+
+	    else
+	      try
+		let pat,subst = choose_subst occ_subterm occ_sol m in
+		let tr_step = AAC_matcher.Subst.instantiate subst pat in
+		let tr_step_raw = AAC_theory.Trans.raw_constr_of_t ir rewinfo.morph_rlt [] tr_step in
+		
+		let conv = (AAC_theory.Trans.raw_constr_of_t ir rewinfo.morph_rlt (hypinfo.AAC_coq.Rewrite.context)) in
+		let subst  = AAC_matcher.Subst.to_list subst in
+		let subst = List.map (fun (x,y) -> x, conv y) subst in
+		let by_aac_reflexivity = (by_aac_reflexivity rewinfo.subject rewinfo.eqt  ir) in
+		core_aac_rewrite ?abort rewinfo subst by_aac_reflexivity tr_step_raw tr_step subject
+		 
+	      with
+		| NoSolutions ->
+		  Tacticals.tclFAIL 0
+		    (Pp.str (if occ_subterm = None && occ_sol = None
+		      then "No matching occurence modulo AC found"
+		      else "No such solution"))
+	)   
+    ) goal
+
+
+open Rewrite
+open Tacmach
+open Tacticals
+open Tacexpr
+open Tacinterp
+open Extraargs
+open Genarg
+
+let rec add k x = function
+  | [] -> [k,x]
+  | k',_ as ky::q ->
+      if k'=k then AAC_coq.user_error ("redondant argument ("^k^")")
+      else ky::add k x q
+
+let get k l = try Some (List.assoc k l) with Not_found -> None
+
+let get_lhs l = try List.assoc "in_right" l; false with Not_found -> true
+
+let aac_rewrite ~args =
+  aac_rewrite ~occ_subterm:(get "at" args) ~occ_sol:(get "subst" args) ~in_left:(get_lhs args)
+
+
+let pr_aac_args _ _ _ l =
+  List.fold_left
+    (fun acc -> function
+       | ("in_right" as s,_) -> Pp.(++) (Pp.str s) acc
+       | (k,i) -> Pp.(++) (Pp.(++) (Pp.str k)  (Pp.int i)) acc
+    ) (Pp.str "") l
+
+ARGUMENT EXTEND aac_args  
+TYPED AS ((string * int) list ) 
+PRINTED BY pr_aac_args
+| [ "at" integer(n) aac_args(q) ] -> [ add "at" n q ]
+| [ "subst" integer(n) aac_args(q) ] -> [ add "subst" n q ]
+| [ "in_right" aac_args(q) ] -> [ add "in_right" 0 q ]
+| [ ] -> [ [] ]
+END
+
+let pr_constro _ _ _ = fun b ->
+  match b with
+    | None ->  Pp.str ""
+    | Some o -> Pp.str "<constr>"
+
+ARGUMENT EXTEND constro
+TYPED AS (constr option) 
+PRINTED BY pr_constro
+| [ "[" constr(c) "]" ] -> [ Some c ]
+| [ ] -> [ None ]
+END
+
+TACTIC EXTEND _aac_reflexivity_
+| [ "aac_reflexivity" ] -> [ aac_reflexivity ]
+END
+
+TACTIC EXTEND _aac_normalise_
+| [ "aac_normalise" ] -> [ aac_normalise ]
+END
+
+TACTIC EXTEND _aac_rewrite_
+| [ "aac_rewrite" orient(l2r) constr(c) aac_args(args) constro(extra)] ->
+  [ fun gl -> aac_rewrite ?extra ~args ~l2r ~strict:true c gl ]
+END
+ 
+TACTIC EXTEND _aac_pattern_
+| [ "aac_pattern" orient(l2r) constr(c) aac_args(args) constro(extra)] ->
+  [ fun gl -> aac_rewrite ?extra ~args ~l2r ~strict:true ~abort:true c gl ]
+END
+
+TACTIC EXTEND _aac_instances_
+| [ "aac_instances" orient(l2r) constr(c) aac_args(args) constro(extra)] ->
+  [ fun gl -> aac_rewrite ?extra ~args ~l2r ~strict:true ~show:true c gl ]
+END
+
+TACTIC EXTEND _aacu_rewrite_
+| [ "aacu_rewrite" orient(l2r) constr(c) aac_args(args) constro(extra)] ->
+  [ fun gl -> aac_rewrite ?extra ~args ~l2r ~strict:false c gl ]
+END
+ 
+TACTIC EXTEND _aacu_pattern_
+| [ "aacu_pattern" orient(l2r) constr(c) aac_args(args) constro(extra)] ->
+  [ fun gl -> aac_rewrite ?extra ~args ~l2r ~strict:false ~abort:true c gl ]
+END
+
+TACTIC EXTEND _aacu_instances_
+| [ "aacu_instances" orient(l2r) constr(c) aac_args(args) constro(extra)] ->
+  [ fun gl -> aac_rewrite ?extra ~args ~l2r ~strict:false ~show:true c gl ]
+END
