AAC_theory.mli
@@ -7,8 +7,8 @@
 (***************************************************************************)
 
 (** Bindings for Coq constants that are specific to the plugin;
-    reification and translation functions. 
-    
+    reification and translation functions.
+   
     Note: this module is highly correlated with the definitions of {i
     AAC.v}.
 
@@ -20,15 +20,22 @@
     AAC.v}).
 *)
 
+(** Both in OCaml and Coq, we represent finite multisets using
+    weighted lists ([('a*int) list]), see {!AAC_matcher.mset}.
 
+    [mk_mset ty l] constructs a Coq multiset from an OCaml multiset
+    [l] of Coq terms of type [ty] *)
 
+val mk_mset:Term.constr -> (Term.constr * int) list ->Term.constr
+
+(** {2 Packaging modules} *)
 
 (** Environments *)
 module Sigma:
 sig
   (**  [add ty n x map] adds the value [x] of type [ty] with key [n] in [map]  *)
   val add: Term.constr ->Term.constr ->Term.constr ->Term.constr ->Term.constr
-    
+   
   (** [empty ty] create an empty map of type [ty]  *)
   val empty: Term.constr ->Term.constr
 
@@ -39,19 +46,6 @@ sig
   val to_fun: Term.constr ->Term.constr ->Term.constr ->Term.constr
 end
 
-(** The constr associated with our typeclasses for AC or A operators *)
-val op_ac:Term.constr lazy_t
-val op_a:Term.constr lazy_t
-  
-(** The evaluation fonction, used to convert a reified coq term to a
-    raw coq term *)
-val eval: Term.constr lazy_t
-  
-(** The main lemma of our theory, that is 
-    [compare (norm u) (norm v) = Eq -> eval u == eval v] *)
-val decide_thm:Term.constr lazy_t
-
-(** {2 Packaging modules} *)
 
 (** Dynamically typed morphisms *)
 module Sym:
@@ -61,80 +55,48 @@ sig
 
   val typ: Term.constr lazy_t
 
-  (** [mk_typeof rlt int]  *)
-  val mk_typeof: Coq.reltype ->int ->Term.constr
-
-  (** [mk_typeof rlt int]  *)
-  val mk_relof:  Coq.reltype ->int ->Term.constr
 
   (** [mk_pack rlt (ar,value,morph)]  *)
-  val mk_pack: Coq.reltype -> pack -> Term.constr
-    
-  (** [null] builds a dummy symbol, given an {!Coq.eqtype} and a
-      constant *)
-  val null: Coq.eqtype -> Term.constr -> Term.constr
-  
-end
-
-(** Dynamically typed AC operations *)
-module Sum:
-sig
-
-  (** mimics the Coq record [Sum.pack] *)
-  type pack = {plus : Term.constr; zero: Term.constr ; opac: Term.constr}
-
-  val typ: Term.constr lazy_t
-
-  (** [mk_pack rlt (plus,zero,opac)]  *)
-  val mk_pack: Coq.reltype -> pack -> Term.constr
-    
-  (** [zero rlt pack]*)
-  val zero: Coq.reltype -> Term.constr -> Term.constr
-
-  (** [plus rlt pack]*)
-  val plus: Coq.reltype -> Term.constr -> Term.constr
-
+  val mk_pack: AAC_coq.Relation.t -> pack -> Term.constr
+   
+  (** [null] builds a dummy (identity) symbol, given an {!AAC_coq.Relation.t} *)
+  val null: AAC_coq.Relation.t -> Term.constr
+ 
 end
 
 
-(** Dynamically typed A operations *)
-module Prd:
-sig
+(** We need to export some Coq stubs out of this module. They are used
+    by the main tactic, see {!AAC_rewrite} *)
+module Stubs : sig
+  val lift : Term.constr Lazy.t
+  val lift_proj_equivalence : Term.constr Lazy.t
+  val lift_transitivity_left : Term.constr Lazy.t
+  val lift_transitivity_right : Term.constr Lazy.t
+  val lift_reflexivity : Term.constr Lazy.t
+    (** The evaluation fonction, used to convert a reified coq term to a
+	raw coq term *)
+  val eval: Term.constr lazy_t
+   
+  (** The main lemma of our theory, that is
+      [compare (norm u) (norm v) = Eq -> eval u == eval v] *)
+  val decide_thm:Term.constr lazy_t 
 
-  (** mimics the Coq record [Prd.pack] *)
-  type pack = {dot: Term.constr; one: Term.constr ; opa: Term.constr}
-
-  val typ: Term.constr lazy_t
-
-  (** [mk_pack rlt (dot,one,opa)]  *)
-  val mk_pack: Coq.reltype -> pack -> Term.constr
-    
-  (** [one rlt pack]*)
-  val one: Coq.reltype -> Term.constr -> Term.constr
-
-  (** [dot rlt pack]*)
-  val dot: Coq.reltype -> Term.constr -> Term.constr
-    
+  val lift_normalise_thm : Term.constr lazy_t
 end
-
-
-(** [mk_equal rlt l r] builds the term [l == r] *)
-val mk_equal : Coq.reltype -> Term.constr -> Term.constr -> Term.constr
-
 
 (** {2 Building reified terms}
-    
+   
     We define a bundle of functions to build reified versions of the
     terms (those that will be given to the reflexive decision
     procedure). In particular, each field takes as first argument the
     index of the symbol rather than the symbol itself. *)
-  
+ 
 (** Tranlations between Coq and OCaml  *)
 module Trans :  sig
 
   (** This module provides facilities to interpret a term with
       arbitrary operators as an instance of an abstract syntax tree
-      {!Matcher.Terms.t}. 
+      {!AAC_matcher.Terms.t}.
 
       For each Coq application [f x_1 ... x_n], this amounts to
       deciding whether one of the partial applications [f x_1
@@ -143,77 +105,93 @@ module Trans :  sig
       whether the whole term is the unit for some A or AC operator. We
       use typeclass resolution to test each of these possibilities.
 
-      Note that there are ambiguous terms: 
+      Note that there are ambiguous terms:
       - a term like [f x y] might yield a unary morphism ([f x]) and a
       binary one ([f]); we select the latter one (unless [f] is A or
       AC, in which case we declare it accordingly);
-      - a term like [S O] can be considered as a morphism ([S]) 
-      applied to a unit for [(+)], or as a unit for [( * )]; we 
-      chose to give priority to units, so that the latter 
-      interpretation is selected in this case;  
-      - an element might be the unit for several operations; the
-      behaviour in this case is almost unspecified: we simply give
-      priority to AC operations.
+      - a term like [S O] can be considered as a morphism ([S])
+      applied to a unit for [(+)], or as a unit for [( * )]; we
+      chose to give priority to units, so that the latter
+      interpretation is selected in this case; 
+      - an element might be the unit for several operations
   *)
-  
-
+ 
   (** To achieve this reification, one need to record informations
       about the collected operators (symbols, binary operators,
       units). We use the following imperative internal data-structure to
       this end. *)
-  
-  type envs 
+ 
+  type envs
   val empty_envs : unit -> envs
+   
 
-  (** {1 Reification: from Coq terms to AST {!Matcher.Terms.t}  } *)
+  (** {2 Reification: from Coq terms to AST {!AAC_matcher.Terms.t}  } *)
 
-  (** [t_of_constr goal rlt envs cstr] builds the abstract syntax tree
-      of the term [cstr]. We rely on the [goal] to perform typeclasses
-      resolutions to find morphisms compatible with the relation
-      [rlt]. Doing so, it modifies the reification environment
-      [envs]. Moreover, we need to create creates fresh evars; this is
-      why we give back the [goal], accordingly updated. *)
-  val t_of_constr : Coq.goal_sigma -> Coq.reltype -> envs -> Term.constr -> Matcher.Terms.t * Coq.goal_sigma
 
-  (** {1 Reconstruction: from AST back to Coq terms  }
-      
+  (** [t_of_constr goal rlt envs (left,right)] builds the abstract
+      syntax tree of the terms [left] and [right]. We rely on the [goal]
+      to perform typeclasses resolutions to find morphisms compatible
+      with the relation [rlt]. Doing so, it modifies the reification
+      environment [envs]. Moreover, we need to create fresh
+      evars; this is why we give back the [goal], accordingly
+      updated. *)
+  
+  val t_of_constr : AAC_coq.goal_sigma -> AAC_coq.Relation.t -> envs -> (Term.constr * Term.constr) -> AAC_matcher.Terms.t * AAC_matcher.Terms.t * AAC_coq.goal_sigma
+
+  (** [add_symbol] adds a given binary symbol to the environment of
+      known stuff. *)
+  val add_symbol : AAC_coq.goal_sigma -> AAC_coq.Relation.t -> envs -> Term.constr -> AAC_coq.goal_sigma
+
+  (** {2 Reconstruction: from AST back to Coq terms  }
+     
       The next functions allow one to map OCaml abstract syntax trees
       to Coq terms. We need two functions to rebuild different kind of
       terms: first, raw terms, like the one encountered by
       {!t_of_constr}; second, reified Coq terms, that are required for
       the reflexive decision procedure. *)
 
-  (** {2 Building raw, natural, terms} *)
+  type ir
+  val ir_of_envs : AAC_coq.goal_sigma -> AAC_coq.Relation.t -> envs -> AAC_coq.goal_sigma * ir
+  val ir_to_units : ir -> AAC_matcher.ext_units
 
-  (** [raw_constr_of_t] rebuilds a term in the raw representation *)
-  val raw_constr_of_t : envs -> Coq.reltype -> Matcher.Terms.t -> Term.constr
+  (** {2 Building raw, natural, terms} *)
+       
+  (** [raw_constr_of_t] rebuilds a term in the raw representation, and
+      reconstruct the named products on top of it. In particular, this
+      allow us to print the context put around the left (or right)
+      hand side of a pattern. *)
+  val raw_constr_of_t : ir ->  AAC_coq.Relation.t -> (Term.rel_context)  ->AAC_matcher.Terms.t -> Term.constr
 
   (** {2 Building reified terms} *)
- 
+
   (** The reification environments, as Coq constrs *)
+
   type sigmas = {
     env_sym : Term.constr;
-    env_sum : Term.constr;
-    env_prd : Term.constr;
+    env_bin : Term.constr;
+    env_units : Term.constr; 		(* the [idx -> X:constr] *)
   }
+    
+
 
   (** We need to reify two terms (left and right members of a goal)
       that share the same reification envirnoment. Therefore, we need
       to add letins to the proof context in order to ensure some
-      sharing in the proof terms we produce. 
+      sharing in the proof terms we produce.
 
       Moreover, in order to have as much sharing as possible, we also
       add letins for various partial applications that are used
       throughout the terms.
-      
+     
       To achieve this, we decompose the reconstruction function into
       two steps: first, we build the reification environment and then
       reify each term successively.*)
   type reifier
 
-  val mk_reifier : Coq.eqtype -> envs -> Coq.goal_sigma -> sigmas * reifier * Proof_type.tactic 
+  val mk_reifier :   AAC_coq.Relation.t -> Term.constr -> ir -> (sigmas * reifier -> Proof_type.tactic) -> Proof_type.tactic
 
   (** [reif_constr_of_t  reifier t] rebuilds the term [t] in the
       reified form. *)
-  val reif_constr_of_t : reifier -> Matcher.Terms.t -> Term.constr
+  val reif_constr_of_t : reifier -> AAC_matcher.Terms.t -> Term.constr
+
 end
