AAC.v
@@ -13,35 +13,35 @@
    quoted) expressions (with morphisms).
 
    We then define a reflexive decision procedure to decide the
-   equality of reified terms: first normalize reified terms, then
+   equality of reified terms: first normalise reified terms, then
    compare them. This allows us to close transitivity steps
    automatically, in the [aac_rewrite] tactic.
-   
+  
    We restrict ourselves to the case where all symbols operate on a
    single fixed type. In particular, this means that we cannot handle
-   situations like   
+   situations like  
 
    [H: forall x y, nat_of_pos (pos_of_nat (x) + y) + x = ....]
 
-   where one occurence of [+] operates on nat while the other one
+   where one occurrence of [+] operates on nat while the other one
    operates on positive. *)
 
-Require Import Arith NArith. 
+Require Import Arith NArith.
 Require Import List.
 Require Import FMapPositive FMapFacts.
 Require Import RelationClasses Equality.
 Require Export Morphisms.
 
 Set Implicit Arguments.
-Unset Automatic Introduction.
-Open Scope signature_scope.
+
+Local Open Scope signature_scope.
 
 (** * Environments for the reification process: we use positive maps to index elements *)
 
 Section sigma.
   Definition sigma := PositiveMap.t.
   Definition sigma_get A (null : A) (map : sigma A) (n : positive) : A :=
-    match PositiveMap.find n map with 
+    match PositiveMap.find n map with
       | None => null
       | Some x => x
     end.
@@ -49,123 +49,78 @@ Section sigma.
   Definition sigma_empty := @PositiveMap.empty.
 End sigma.
 
-(** * Packaging structures *)
 
-(** ** Free symbols  *)
-Module Sym.
-  Section t.
-  Context {X} {R : relation X} .
-  
-  (** type of an arity  *)
-  Fixpoint type_of  (n: nat) :=
-  match n with
-    | O => X
-    | S n => X -> type_of  n
-  end.
+(** * Classes for properties of operators *)
 
-  (** relation to be preserved at an arity  *)
-  Fixpoint rel_of n : relation (type_of n) := 
-    match n with
-      | O => R
-      | S n => respectful R (rel_of n)
-    end.
-  
-  (** a symbol package contains an arity, 
-     a value of the corresponding type, 
-     and a proof that the value is a proper morphism *)
-  Record pack  : Type := mkPack {
-    ar : nat;
-    value : type_of  ar;
-    morph : Proper (rel_of ar) value
-  }.
-
-  (** helper to build default values, when filling reification environments *)
-  Program Definition null (H: Equivalence R) (x : X)  := mkPack 0 x _.
-    
-  End t.
-
-End Sym.
-
-(** ** Associative commutative operations (commutative monoids) 
-   
-   See #<a href="Instances.html">Instances.v</a># for concrete instances of these classes.
-
-*)
-
-Class Op_AC (X:Type) (R: relation X) (plus: X -> X -> X) (zero:X) := {
-  plus_compat:> Proper (R ==> R ==> R) plus;
-  plus_neutral_left: forall x, R (plus zero x) x;
-  plus_assoc: forall x y z, R (plus x (plus y z)) (plus (plus x y) z);
-  plus_com: forall x y, R (plus x y) (plus y x)
-}.
-
-Module Sum.
-  Section t.
-  Context {X : Type} {R: relation X}.
-  Class pack : Type := mkPack {
-    plus : X -> X -> X;
-    zero : X;
-    opac :> @Op_AC X R plus zero
-  }.
-  End t.
-End Sum.
-  
-    
-
-(** ** Associative operations (monoids) *)
-Class Op_A (X:Type) (R:relation X) (dot: X -> X -> X) (one: X) := {
-  dot_compat:> Proper (R ==> R ==> R) dot;
-  dot_neutral_left: forall x, R (dot one x) x;
-  dot_neutral_right: forall x, R (dot x one) x;
-  dot_assoc: forall x y z, R (dot x (dot y z)) (dot (dot x y) z)
+Class Associative (X:Type) (R:relation X) (dot: X -> X -> X) :=
+  law_assoc : forall x y z, R (dot x (dot y z)) (dot (dot x y) z).
+Class Commutative (X:Type) (R: relation X) (plus: X -> X -> X) :=
+  law_comm: forall x y, R (plus x y) (plus y x).
+Class Unit (X:Type) (R:relation X) (op : X -> X -> X) (unit:X) := {
+  law_neutral_left: forall x, R (op unit x) x;
+  law_neutral_right: forall x, R (op x unit) x
 }.
 
 
-Module Prd.
-  Section t.
-  Context {X : Type} {R: relation X}.
-  Class pack : Type := mkPack {
-    dot : X -> X -> X;
-    one : X;
-    opa :> @Op_A X R dot one
-  }.
-  End t.
-End Prd.
+(** Class used to find the equivalence relation on which operations
+   are A or AC, starting from the relation appearing in the goal *)
 
+Class AAC_lift X (R: relation X) (E : relation X) := {
+  aac_lift_equivalence : Equivalence E;
+  aac_list_proper : Proper (E ==> E ==> iff) R
+}.
 
-(** an helper lemma to derive an A class out of an AC one (not
-   declared as an instance to avoid useless branches in typeclass
-   resolution) *)
-Lemma AC_A {X} {R:relation X} {EQ: Equivalence R} {plus} {zero} (op: Op_AC R plus zero): Op_A R plus zero.
+(** simple instances, when we have a subrelation, or an equivalence *)
+
+Instance aac_lift_subrelation {X} {R} {E} {HE: Equivalence E}
+  {HR: @Transitive X R} {HER: subrelation E R}: AAC_lift  R E | 3.
 Proof.
-  split; try apply op.
-   intros. rewrite plus_com. apply op.
+  constructor; trivial.
+  intros ? ? H ? ? H'. split; intro G.
+   rewrite <- H, G. apply HER, H'.
+   rewrite H, G. apply HER. symmetry. apply H'.
 Qed.
 
+Instance aac_lift_proper {X} {R : relation X} {E} {HE: Equivalence E}
+  {HR: Proper (E==>E==>iff) R}: AAC_lift  R E | 4.
 
+
+
+Module Internal.
 
 (** * Utilities for the evaluation function *)
+
 Section copy.
 
-  Context  {X} {R: relation X} {HR : @Equivalence X R} {plus} {zero} {op: @Op_AC X R plus zero}.
+  Context {X} {R} {HR: @Equivalence X R} {plus}
+   (op: Associative R plus) (op': Commutative R plus) (po: Proper (R ==> R ==> R) plus).
 
   (* copy n x = x+...+x (n times) *)
-  Definition copy n x := Prect (fun _ => X) x (fun _ xn => plus x xn) n.
-  
+  Fixpoint copy' n x := match n with
+                         | xH => x
+                         | xI n => let xn := copy' n x in plus (plus xn xn) x
+                         | xO n => let xn := copy' n x in (plus xn xn)
+                       end.
+  Definition copy n x :=  Prect (fun _ => X) x (fun _ xn => plus x xn) n.
+     
   Lemma copy_plus : forall n m x, R (copy (n+m) x) (plus (copy n x) (copy m x)).
   Proof.
     unfold copy.
     induction n using Pind; intros m x.
-     rewrite Prect_base. rewrite <- Pplus_one_succ_l. rewrite Prect_succ. reflexivity.
-     rewrite Pplus_succ_permute_l. rewrite 2Prect_succ. rewrite IHn. apply plus_assoc. 
+     rewrite Prect_base. rewrite <- Pplus_one_succ_l. rewrite Prect_succ. reflexivity. 
+     rewrite Pplus_succ_permute_l. rewrite 2Prect_succ. rewrite IHn. apply op.
   Qed.
+  Lemma copy_xH : forall x, R (copy 1 x) x.
+  Proof. intros; unfold copy; rewrite Prect_base. reflexivity. Qed.
+  Lemma copy_Psucc : forall n x, R (copy (Psucc n) x) (plus x (copy n x)).
+  Proof. intros; unfold copy; rewrite Prect_succ. reflexivity. Qed.
 
   Global Instance copy_compat n: Proper (R ==> R) (copy n).
   Proof.
     unfold copy.
     induction n using Pind; intros x y H.
-     rewrite 2Prect_base. assumption. 
-     rewrite 2Prect_succ. apply plus_compat; auto. 
+     rewrite 2Prect_base. assumption.
+     rewrite 2Prect_succ. apply po; auto.
   Qed.
 
 End copy.
@@ -173,12 +128,12 @@ End copy.
 (** * Utilities for positive numbers
    which we use as:
      - indices for morphisms and symbols
-     - multiplicity of terms in sums
- *)
-Notation idx := positive.
+     - multiplicity of terms in sums *)
+
+Local Notation idx := positive.
 
 Fixpoint eq_idx_bool i j :=
-  match i,j with 
+  match i,j with
     | xH, xH => true
     | xO i, xO j => eq_idx_bool i j
     | xI i, xI j => eq_idx_bool i j
@@ -186,7 +141,7 @@ Fixpoint eq_idx_bool i j :=
   end.
 
 Fixpoint idx_compare i j :=
-  match i,j with 
+  match i,j with
     | xH, xH => Eq
     | xH, _ => Lt
     | _, xH => Gt
@@ -196,9 +151,9 @@ Fixpoint idx_compare i j :=
     | xO _, xI _ => Lt
   end.
 
-Notation pos_compare := idx_compare (only parsing).
+Local Notation pos_compare := idx_compare (only parsing).
 
-(** specification predicate for boolean binary functions *)
+(** Specification predicate for boolean binary functions *)
 Inductive decide_spec {A} {B} (R : A -> B -> Prop) (x : A) (y : B) : bool -> Prop :=
 | decide_true : R x y -> decide_spec R x y true
 | decide_false : ~(R x y) -> decide_spec R x y false.
@@ -208,7 +163,7 @@ Proof.
   induction i; destruct j; simpl; try (constructor; congruence).
    case (IHi j); constructor; congruence.
    case (IHi j); constructor; congruence.
-Qed. 
+Qed.
 
 (** weak specification predicate for comparison functions: only the 'Eq' case is specified *)
 Inductive compare_weak_spec A: A -> A -> comparison -> Prop :=
@@ -222,27 +177,29 @@ Proof. induction i; destruct j; simpl; try constructor; case (IHi j); intros; co
 Lemma idx_compare_reflect_eq: forall i j, idx_compare i j = Eq -> i=j.
 Proof. intros i j. case (pos_compare_weak_spec i j); intros; congruence. Qed.
 
-
 (** * Dependent types utilities *)
-Notation cast T H u := (eq_rect _ T u _ H).
+
+Local Notation cast T H u := (eq_rect _ T u _ H).
 
 Section dep.
   Variable U: Type.
   Variable T: U -> Type.
 
-  Lemma cast_eq: (forall u v: U, {u=v}+{u<>v}) -> 
+  Lemma cast_eq: (forall u v: U, {u=v}+{u<>v}) ->
     forall A (H: A=A) (u: T A), cast T H u = u.
-  Proof. intros. rewrite <- Eqdep_dec.eq_rect_eq_dec; trivial. Qed. 
+  Proof. intros. rewrite <- Eqdep_dec.eq_rect_eq_dec; trivial. Qed.
 
   Variable f: forall A B, T A -> T B -> comparison.
   Definition reflect_eqdep := forall A u B v (H: A=B), @f A B u v = Eq -> cast T H u = v.
 
   (* these lemmas have to remain transparent to get structural recursion
      in the lemma [tcompare_weak_spec] below *)
-  Lemma reflect_eqdep_eq: reflect_eqdep -> forall A u v, @f A A u v = Eq -> u = v.
-  Proof. intros H A u v He. apply (H _ _ _ _ eq_refl He). Defined. 
+  Lemma reflect_eqdep_eq: reflect_eqdep ->
+    forall A u v, @f A A u v = Eq -> u = v.
+  Proof. intros H A u v He. apply (H _ _ _ _ eq_refl He). Defined.
 
-  Lemma reflect_eqdep_weak_spec: reflect_eqdep -> forall A u v, compare_weak_spec u v (@f A A u v).
+  Lemma reflect_eqdep_weak_spec: reflect_eqdep ->
+    forall A u v, compare_weak_spec u v (@f A A u v).
   Proof.
     intros. case_eq (f u v); try constructor.
     intro H'. apply reflect_eqdep_eq in H'. subst. constructor. assumption.
@@ -250,42 +207,70 @@ Section dep.
 End dep.
 
 
-(** * Utilities about lists and multisets  *)
+
+(** * Utilities about (non-empty) lists and multisets  *)
+
+Inductive nelist (A : Type) : Type :=
+| nil : A -> nelist A
+| cons : A -> nelist A -> nelist A.
+
+Local Notation "x :: y" := (cons x y).
+
+Fixpoint nelist_map (A B: Type) (f: A -> B) l :=
+  match l with
+    | nil x => nil ( f x)
+    | cons x l => cons ( f x) (nelist_map  f l)
+  end.
+
+Fixpoint appne  A l l' : nelist A :=
+  match l with
+    nil x => cons x l'
+    | cons t q => cons t (appne A q l')
+  end.
+
+Local Notation "x ++ y" := (appne x y).
 
 (** finite multisets are represented with ordered lists with multiplicities *)
-Definition mset A := list (A*positive).
+Definition mset A := nelist (A*positive).
 
 (** lexicographic composition of comparisons (this is a notation to keep it lazy) *)
-Notation lex e f := (match e with Eq => f | _ => e end).   
+Local Notation lex e f := (match e with Eq => f | _ => e end).  
 
 
 Section lists.
 
-  (** comparison function  *)
+  (** comparison functions *)
+
   Section c.
     Variables A B: Type.
     Variable compare: A -> B -> comparison.
-    Fixpoint list_compare h k := 
+    Fixpoint list_compare h k :=
       match h,k with
-        | nil, nil => Eq
-        | nil, _   => Lt
-        | _,   nil => Gt
-      | u::h, v::k => lex (compare u v) (list_compare h k)
-      end.  
+        | nil x, nil y => compare x y
+        | nil x, _   => Lt
+        | _,   nil x => Gt
+        | u::h, v::k => lex (compare u v) (list_compare h k)
+      end. 
   End c.
   Definition mset_compare A B compare: mset A -> mset B -> comparison :=
-    list_compare (fun un vm => let '(u,n) := un in let '(v,m) := vm in lex (compare u v) (pos_compare n m)).
+    list_compare (fun un vm =>
+      let '(u,n) := un in
+        let '(v,m) := vm in
+          lex (compare u v) (pos_compare n m)).
 
   Section list_compare_weak_spec.
     Variable A: Type.
     Variable compare: A -> A -> comparison.
     Hypothesis Hcompare: forall u v, compare_weak_spec u v (compare u v).
-    (* this lemma has to remain transparent to get structural recursion 
+    (* this lemma has to remain transparent to get structural recursion
        in the lemma [tcompare_weak_spec] below *)
-    Lemma list_compare_weak_spec: forall h k, compare_weak_spec h k (list_compare compare h k).
+    Lemma list_compare_weak_spec: forall h k,
+      compare_weak_spec h k (list_compare compare h k).
     Proof.
       induction h as [|u h IHh]; destruct k as [|v k]; simpl; try constructor.
-      case (Hcompare u v); try constructor.
+
+      case (Hcompare a a0 ); try constructor.
+      case (Hcompare u v ); try constructor.
       case (IHh k); intros; constructor.
     Defined.
   End list_compare_weak_spec.
@@ -294,9 +279,10 @@ Section lists.
     Variable A: Type.
     Variable compare: A -> A -> comparison.
     Hypothesis Hcompare: forall u v, compare_weak_spec u v (compare u v).
-    (* this lemma has to remain transparent to get structural recursion 
+    (* this lemma has to remain transparent to get structural recursion
        in the lemma [tcompare_weak_spec] below *)
-    Lemma mset_compare_weak_spec: forall h k, compare_weak_spec h k (mset_compare compare h k).
+    Lemma mset_compare_weak_spec: forall h k,
+      compare_weak_spec h k (mset_compare compare h k).
     Proof.
       apply list_compare_weak_spec.
       intros [u n] [v m].
@@ -306,17 +292,40 @@ Section lists.
   End mset_compare_weak_spec.
 
   (** (sorted) merging functions  *)
+
   Section m.
     Variable A: Type.
     Variable compare: A -> A -> comparison.
-
+    Definition insert n1 h1 :=
+      let fix insert_aux l2 :=
+      match l2 with
+        | nil (h2,n2) =>
+          match compare h1 h2 with
+            | Eq => nil (h1,Pplus n1 n2)
+            | Lt => (h1,n1):: nil (h2,n2)
+            | Gt => (h2,n2):: nil (h1,n1)
+          end
+        | (h2,n2)::t2 =>
+          match compare h1 h2 with
+            | Eq => (h1,Pplus n1 n2):: t2
+            | Lt => (h1,n1)::l2
+            | Gt => (h2,n2)::insert_aux t2
+          end
+      end
+      in insert_aux.
+   
     Fixpoint merge_msets l1 :=
       match l1 with
-        | nil => fun l2 => l2
+        | nil (h1,n1) => fun l2 => insert n1 h1 l2
         | (h1,n1)::t1 =>
           let fix merge_aux l2 :=
             match l2 with
-              | nil => l1
+               | nil (h2,n2) =>
+                match compare h1 h2 with
+                  | Eq => (h1,Pplus n1 n2) :: t1
+                  | Lt => (h1,n1):: merge_msets t1 l2
+                  | Gt => (h2,n2)::  l1
+                end
               | (h2,n2)::t2 =>
                 match compare h1 h2 with
                   | Eq => (h1,Pplus n1 n2)::merge_msets t1 t2
@@ -328,44 +337,119 @@ Section lists.
       end.
 
     (** interpretation of a list with a constant and a binary operation *)
+
     Variable B: Type.
     Variable map: A -> B.
     Variable b2: B -> B -> B.
-    Variable b0: B.
     Fixpoint fold_map l :=
       match l with
-        | nil => b0
-        | u::nil => map u
+        | nil x => map x
         | u::l => b2 (map u) (fold_map l)
       end.
 
     (** mapping and merging *)
-    Variable merge: A -> list B -> list B.
-    Fixpoint merge_map (l: list A): list B :=
+
+    Variable merge: A -> nelist B -> nelist B.
+    Fixpoint merge_map (l: nelist A): nelist B :=
       match l with
-        | nil => nil
+        | nil x => nil (map x)
         | u::l => merge u (merge_map l)
       end.
 
-  End m.
+    Variable ret : A -> B.
+    Variable bind : A -> B -> B.
+    Fixpoint fold_map' (l : nelist A) : B :=
+      match l with
+        | nil x => ret x
+        | u::l => bind u (fold_map' l)
+      end.
 
+  End m.
 End lists.
 
+(** * Packaging structures *)
+
+(** ** free symbols  *)
+
+Module Sym.
+  Section t.
+    Context {X} {R : relation X} .
+   
+    (** type of an arity  *)
+    Fixpoint type_of  (n: nat) :=
+      match n with
+        | O => X
+        | S n => X -> type_of  n
+      end.
+
+    (** relation to be preserved at an arity  *)
+    Fixpoint rel_of n : relation (type_of n) :=
+      match n with
+        | O => R
+      | S n => respectful R (rel_of n)
+      end.
+   
+  (** a symbol package contains an arity,
+     a value of the corresponding type,
+     and a proof that the value is a proper morphism *)
+  Record pack  : Type := mkPack {
+    ar : nat;
+    value :> type_of  ar;
+    morph : Proper (rel_of ar) value
+  }.
+
+  (** helper to build default values, when filling reification environments *)
+  Definition null: pack := mkPack 1 (fun x => x) (fun _ _ H => H).
+   
+  End t.
+
+End Sym.
+  
+(** ** binary operations *)
+
+Module Bin.
+  Section t.
+    Context {X} {R: relation X}.
+
+    Record pack := mk_pack {
+      value:> X -> X -> X;
+      compat: Proper (R ==> R ==> R) value;
+      assoc: Associative R value;
+      comm: option (Commutative R value)
+    }.
+  End t.
+  (*    See #<a href="Instances.html">Instances.v</a># for concrete instances of these classes. *)
+
+End Bin.
 
 
 (** * Reification, normalisation, and decision  *)
+
 Section s.
   Context {X} {R: relation X} {E: @Equivalence X R}.
   Infix "==" := R (at level 80).
 
   (* We use environments to store the various operators and the
      morphisms.*)
-
+ 
   Variable e_sym: idx -> @Sym.pack X R.
-  Variable e_prd: idx -> @Prd.pack X R.
-  Variable e_sum: idx -> @Sum.pack X R.
-  Hint Resolve e_sum e_prd: typeclass_instances.
+  Variable e_bin: idx -> @Bin.pack X R.
 
+ 
+  (** packaging units (depends on e_bin) *)
+
+  Record unit_of u := mk_unit_for {
+    uf_idx: idx;
+    uf_desc: Unit R (Bin.value (e_bin uf_idx)) u
+  }.
+
+  Record unit_pack := mk_unit_pack {
+    u_value:> X;
+    u_desc: list (unit_of u_value)
+  }.
+  Variable e_unit: positive -> unit_pack.
+ 
+  Hint Resolve e_bin e_unit: typeclass_instances.
 
   (** ** Almost normalised syntax
      a term in [T] is in normal form if:
@@ -373,16 +457,18 @@ Section s.
      - products do not contain products
      - there are no unary sums or products
      - lists and msets are lexicographically sorted according to the order we define below
-     
-     [vT n] denotes the set of term vectors of size [n] (the mutual dependency could be removed), 
+    
+     [vT n] denotes the set of term vectors of size [n] (the mutual dependency could be removed),
 
      Note that [T] and [vT] depend on the [e_sym] environment (which
      contains, among other things, the arity of symbols)
      *)
-  Inductive T: Type := 
+
+  Inductive T: Type :=
   | sum: idx -> mset T -> T
-  | prd: idx -> list T -> T
+  | prd: idx -> nelist T -> T
   | sym: forall i, vT (Sym.ar (e_sym i)) -> T
+  | unit : idx -> T
   with vT: nat -> Type :=
   | vnil: vT O
   | vcons: forall n, T -> vT n -> vT (S n).
@@ -390,14 +476,18 @@ Section s.
 
   (** lexicographic rpo over the normalised syntax *)
   Fixpoint compare (u v: T) :=
-    match u,v with 
+    match u,v with
       | sum i l, sum j vs => lex (idx_compare i j) (mset_compare compare l vs)
       | prd i l, prd j vs => lex (idx_compare i j) (list_compare compare l vs)
       | sym i l, sym j vs => lex (idx_compare i j) (vcompare l vs)
+      | unit i , unit j => idx_compare i j
+      | unit _ , _        => Lt
+      | _      , unit _  => Gt
       | sum _ _, _        => Lt
       | _      , sum _ _  => Gt
       | prd _ _, _        => Lt
       | _      , prd _ _  => Gt
+
     end
   with vcompare i j (us: vT i) (vs: vT j) :=
     match us,vs with
@@ -406,12 +496,27 @@ Section s.
       | _,    vnil => Gt
       | vcons _ u us, vcons _ v vs => lex (compare u v) (vcompare us vs)
     end.
+ 
 
 
-  (** we need to show that compare reflects equality
-     (this is because we work with msets rather than lists with arities) 
-    *)
+  (** ** Evaluation from syntax to the abstract domain *)
 
+  Fixpoint eval u: X :=
+    match u with
+      | sum i l => let o := Bin.value (e_bin i) in
+        fold_map (fun un => let '(u,n):=un in @copy _ o n (eval u)) o l
+      | prd i l => fold_map eval (Bin.value (e_bin i)) l
+      | sym i v => eval_aux v (Sym.value (e_sym i))
+      | unit i  => e_unit i
+    end
+  with eval_aux i (v: vT i): Sym.type_of i -> X :=
+    match v with
+      | vnil => fun f => f
+      | vcons _ u v => fun f => eval_aux v (f (eval u))
+    end.
+
+  (** we need to show that compare reflects equality (this is because
+     we work with msets rather than lists with arities) *)
   Lemma tcompare_weak_spec: forall (u v : T), compare_weak_spec u v (compare u v)
   with vcompare_reflect_eqdep: forall i us j vs (H: i=j), vcompare us vs = Eq -> cast vT H us = vs.
   Proof.
@@ -421,269 +526,610 @@ Section s.
       case (mset_compare_weak_spec compare tcompare_weak_spec m m0); intros; try constructor.
      destruct v; simpl; try constructor.
       case (pos_compare_weak_spec p p0); intros; try constructor.
-      case (list_compare_weak_spec compare tcompare_weak_spec l l0); intros; try constructor.
+      case (list_compare_weak_spec compare tcompare_weak_spec n n0); intros; try constructor.
      destruct v0; simpl; try constructor.
       case_eq (idx_compare i i0); intro Hi; try constructor.
       apply idx_compare_reflect_eq in Hi. symmetry in Hi. subst. (* the [symmetry] is required ! *)
       case_eq (vcompare v v0); intro Hv; try constructor.
-      rewrite <- (vcompare_reflect_eqdep _ _ _ _ eq_refl Hv). constructor. 
+      rewrite <- (vcompare_reflect_eqdep _ _ _ _ eq_refl Hv). constructor.
+     destruct v; simpl; try constructor.
+      case_eq (idx_compare p p0); intro Hi; try constructor.
+      apply idx_compare_reflect_eq in Hi. symmetry in Hi. subst.  constructor.
 
     induction us; destruct vs; simpl; intros H Huv; try discriminate.
-     apply cast_eq, eq_nat_dec. 
+     apply cast_eq, eq_nat_dec.
      injection H; intro Hn.
-     revert Huv; case (tcompare_weak_spec t t0); intros; try discriminate. 
+     revert Huv; case (tcompare_weak_spec t t0); intros; try discriminate.
      symmetry in Hn. subst.   (* symmetry required *)
-     rewrite <- (IHus _ _ eq_refl Huv). 
+     rewrite <- (IHus _ _ eq_refl Huv).
      apply cast_eq, eq_nat_dec.
   Qed.
-
-  (** ** Evaluation from syntax to the abstract domain *)
-  Fixpoint eval u: X :=
-    match u with 
-      | sum i l => fold_map (fun un => let '(u,n):=un in @copy _ (@Sum.plus _ _ (e_sum i)) n (eval u))
-                            (@Sum.plus _ _ (e_sum i)) (@Sum.zero _ _ (e_sum i)) l 
-      | prd i l => fold_map eval 
-                            (@Prd.dot _ _ (e_prd i)) (@Prd.one _ _ (e_prd i)) l 
-      | sym i v => @eval_aux _ v (Sym.value (e_sym i))
-    end
-  with eval_aux i (v: vT i): Sym.type_of  i -> X :=
-    match v with
-      | vnil => fun f => f
-      | vcons _ u v => fun f => eval_aux v (f (eval u))
-    end.
-
 
   Instance eval_aux_compat i (l: vT i): Proper (@Sym.rel_of X R i ==> R) (eval_aux l).
   Proof.
     induction l; simpl; repeat intro.
      assumption.
-     apply IHl, H. reflexivity. 
+     apply IHl, H. reflexivity.
   Qed.
+
+ 
+  (* is [i] a unit for [j] ? *)
+  Definition is_unit_of j i :=
+    List.existsb (fun p => eq_idx_bool j (uf_idx p)) (u_desc (e_unit i)).
+
+  (* is [i] commutative ? *)
+  Definition is_commutative i :=
+    match Bin.comm (e_bin i) with Some _ => true | None => false end.
 
 
   (** ** Normalisation *)
 
-  (** auxiliary functions, to clean up sums and products  *)
-  Definition sum' i (u: mset T): T :=
-    match u with 
-      | (u,xH)::nil => u
-      | _ => sum i u
+  Inductive discr {A} : Type :=
+  | Is_op : A -> discr
+  | Is_unit : idx -> discr
+  | Is_nothing : discr .
+ 
+  (* This is called sum in the std lib *)
+  Inductive m {A} {B} :=
+  | left : A -> m
+  | right : B -> m.
+
+  Definition comp A B (merge : B -> B -> B) (l : B) (l' : @m A B) : @m A B :=
+    match l' with
+      | left _ => right l
+      | right l' => right (merge l l')
     end.
-  Definition is_sum i (u: T): option (mset T) :=
-    match u with 
-      | sum j l => if eq_idx_bool j i then Some l else None
-      | u => None
-    end.
-  Definition copy_mset n (l: mset T): mset T :=
-    match n with 
-      | xH => l
-      | _ => List.map (fun vm => let '(v,m):=vm in (v,Pmult n m)) l
-    end.
-  Definition sum_to_mset i (u: T) n := 
-    match is_sum i u with 
-      | Some l' => copy_mset n l' 
-      | None => (u,n)::nil 
+ 
+  (** auxiliary functions, to clean up sums  *)
+
+  Section sums.
+    Variable i : idx.
+    Variable is_unit : idx -> bool.
+
+    Definition sum' (u: mset T): T :=
+      match u with
+        | nil (u,xH) => u
+        | _ => sum i u
+      end.
+
+    Definition is_sum  (u: T) : @discr (mset T) :=
+    match u with
+      | sum j l => if eq_idx_bool j i then Is_op l else Is_nothing
+      | unit j => if is_unit j   then Is_unit j else Is_nothing
+      | u => Is_nothing
     end.
 
-  Definition prd' i (u: list T): T :=
-    match u with 
-      | u::nil => u
+    Definition copy_mset n (l: mset T): mset T :=
+      match n with
+        | xH => l
+        | _ => nelist_map (fun vm => let '(v,m):=vm in (v,Pmult n m)) l
+      end.
+   
+    Definition return_sum  u n :=
+      match is_sum  u with
+        | Is_nothing => right (nil (u,n))
+        | Is_op l' =>  right (copy_mset n l')
+        | Is_unit j => left j
+      end.
+   
+    Definition add_to_sum u n (l : @m idx (mset T))  :=
+      match is_sum  u with
+        | Is_nothing => comp (merge_msets compare) (nil (u,n)) l
+        | Is_op l' => comp (merge_msets compare) (copy_mset n l') l
+        | Is_unit _ => l
+    end.
+
+
+    Definition norm_msets_ norm  (l: mset T) :=
+    fold_map'
+    (fun un => let '(u,n) := un in  return_sum  (norm u) n)
+    (fun un l => let '(u,n) := un in  add_to_sum  (norm u) n l) l.
+
+
+  End sums.
+ 
+  (** similar functions for products *)
+
+  Section prds.
+
+    Variable i : idx.
+    Variable is_unit : idx -> bool.
+    Definition prd'  (u: nelist T): T :=
+    match u with
+      | nil u => u
       | _ => prd i u
     end.
-  Definition is_prd i (u: T): option (list T) :=
-    match u with 
-      | prd j l => if eq_idx_bool j i then Some l else None
-      | u => None
+
+    Definition is_prd (u: T) : @discr (nelist T) :=
+    match u with
+      | prd j l => if eq_idx_bool j i then Is_op l else Is_nothing
+      | unit j => if is_unit j  then Is_unit j else Is_nothing
+      | u => Is_nothing
     end.
-  Definition prd_to_list i (u: T) := 
-    match is_prd i u with
-      | Some l' => l' 
-      | None => u::nil 
-    end.
+ 
+   
+    Definition return_prd u :=
+      match is_prd u with
+        | Is_nothing => right (nil (u))
+        | Is_op l' =>  right (l')
+        | Is_unit j => left j
+      end.
+   
+    Definition add_to_prd  u  (l : @m idx (nelist T))  :=
+      match is_prd  u with
+        | Is_nothing => comp (@appne T) (nil (u)) l
+        | Is_op l' => comp (@appne T) (l') l
+        | Is_unit _ => l
+      end.
+
+    Definition norm_lists_ norm (l : nelist T) :=
+    fold_map'
+    (fun u => return_prd  (norm u))
+    (fun u l => add_to_prd (norm u) l) l.
 
 
-  (** we deduce the normalisation function *)
-  Fixpoint norm u :=
-    match u with 
-      | sum i l => sum' i (merge_map (fun un l => let '(u,n):=un in 
-                                      merge_msets compare (sum_to_mset i (norm u) n) l) l)
-      | prd i l => prd' i (merge_map (fun u l => prd_to_list i (norm u) ++ l) l)
+  End prds.
+
+
+  Definition run_list x := match x with
+                        | left n => nil (unit n)
+                        | right l => l
+                      end.
+ 
+  Definition norm_lists norm i l :=
+    let is_unit := is_unit_of i in
+      run_list (norm_lists_ i is_unit norm l).
+
+  Definition run_msets x := match x with
+                        | left n => nil (unit n, xH)
+                        | right l => l
+                      end.
+ 
+  Definition norm_msets norm i l :=
+    let is_unit := is_unit_of i in
+      run_msets (norm_msets_ i is_unit norm l).
+ 
+  Fixpoint norm u {struct u}:=
+    match u with
+      | sum i l => if is_commutative i then sum' i (norm_msets norm i l)  else u
+      | prd i l => prd' i (norm_lists norm i l)
       | sym i l => sym i (vnorm l)
+      | unit i => unit i
     end
-  with vnorm i (l: vT i): vT i := 
+  with vnorm i (l: vT i): vT i :=
     match l with
       | vnil => vnil
       | vcons _ u l => vcons (norm u) (vnorm l)
     end.
 
-
   (** ** Correctness *)
 
+  Lemma is_unit_of_Unit  : forall i j : idx,
+   is_unit_of i j = true -> Unit R (Bin.value (e_bin i)) (eval (unit j)).
+  Proof.
+    intros. unfold is_unit_of in H.
+    rewrite existsb_exists in H.
+    destruct H as [x [H H']].
+    revert H' ; case (eq_idx_spec); [intros H' _ ; subst| intros _ H'; discriminate].
+    simpl. destruct x. simpl. auto.
+  Qed.
+ 
+  Instance Binvalue_Commutative i (H :  is_commutative i = true) : Commutative R  (@Bin.value _ _ (e_bin i) ).
+  Proof.
+    unfold is_commutative in H.
+    destruct (Bin.comm (e_bin i)); auto.
+    discriminate.
+  Qed.
+
+  Instance Binvalue_Associative i :Associative R (@Bin.value _ _ (e_bin i) ).
+  Proof.
+    destruct ((e_bin i)); auto.
+  Qed.
+ 
+  Instance Binvalue_Proper i : Proper (R ==> R ==> R) (@Bin.value _ _ (e_bin i) ).
+  Proof.
+    destruct ((e_bin i)); auto.
+  Qed.
+  Hint Resolve Binvalue_Proper Binvalue_Associative Binvalue_Commutative.
+
   (** auxiliary lemmas about sums  *)
-  Lemma sum'_sum i (l: mset T): eval (sum' i l) ==eval (sum i l) .
-  Proof. 
-    intros i [|? [|? ?]].
-     reflexivity.
-     destruct p; destruct p; simpl; reflexivity.
-     destruct p; destruct p; simpl; reflexivity.
-  Qed.
 
-  Lemma eval_sum_cons i n a (l: mset T): 
-    (eval (sum i ((a,n)::l))) == (@Sum.plus _ _ (e_sum i) (@copy _ (@Sum.plus _ _ (e_sum i)) n (eval a)) (eval (sum i l))).
-  Proof.
-    intros i n a [|[b m] l]; simpl. 
-     rewrite plus_com, plus_neutral_left. reflexivity.
-     reflexivity.
-  Qed.        
+  Hint Resolve is_unit_of_Unit.
+  Section sum_correctness.
+    Variable i : idx.
+    Variable is_unit : idx -> bool.
+    Hypothesis is_unit_sum_Unit : forall j, is_unit j = true->  @Unit X R (Bin.value (e_bin i)) (eval (unit j)).
 
-  Lemma eval_sum_app i (h k: mset T):  eval (sum i (h++k)) == @Sum.plus _ _ (e_sum i) (eval (sum i h)) (eval (sum i k)).
-  Proof.
-    induction h; intro k. 
-     simpl. rewrite plus_neutral_left. reflexivity.
-     simpl app. destruct a. rewrite 2 eval_sum_cons, IHh, plus_assoc. reflexivity.
-  Qed.        
+    Inductive is_sum_spec_ind : T ->  @discr (mset T) -> Prop :=
+    | is_sum_spec_op : forall j l, j = i -> is_sum_spec_ind (sum j l) (Is_op l)
+    | is_sum_spec_unit : forall j, is_unit j = true ->  is_sum_spec_ind (unit j) (Is_unit j)
+    | is_sum_spec_nothing : forall u, is_sum_spec_ind  u (Is_nothing).
+ 
+    Lemma is_sum_spec u : is_sum_spec_ind u (is_sum i is_unit u).
+    Proof.
+      unfold is_sum; case u; intros; try constructor.
+      case_eq (eq_idx_bool p i); intros; subst;  try constructor; auto.
+      revert H. case eq_idx_spec; try discriminate. auto.
+      case_eq (is_unit p); intros; try constructor. auto.
+    Qed.
 
-  Lemma eval_merge_sum i (h k: mset T): 
-    eval (sum i (merge_msets compare h k)) == @Sum.plus _ _ (e_sum i) (eval (sum i h)) (eval (sum i k)).
-  Proof.
-    induction h as [|[a n] h IHh]; intro k. 
-     simpl. rewrite plus_neutral_left. reflexivity.
-     induction k as [|[b m] k IHk].
-      simpl. setoid_rewrite plus_com. rewrite plus_neutral_left. reflexivity.
-      simpl merge_msets. rewrite eval_sum_cons. destruct (tcompare_weak_spec a b) as [a|a b|a b]. 
-       rewrite 2eval_sum_cons. rewrite IHh. rewrite <- plus_assoc. setoid_rewrite plus_assoc at 3.
-       setoid_rewrite plus_com at 5. rewrite !plus_assoc. rewrite copy_plus. reflexivity.
+    Instance assoc :   @Associative X R (Bin.value (e_bin i)).
+    Proof.
+      destruct (e_bin i). simpl. assumption.
+    Qed.
+    Instance proper :   Proper (R ==> R ==> R)(Bin.value (e_bin i)).
+    Proof.
+      destruct (e_bin i). simpl. assumption.
+    Qed.
+    Hypothesis comm : @Commutative X R (Bin.value (e_bin i)).
 
-       rewrite eval_sum_cons. rewrite IHh. apply plus_assoc.
+    Lemma sum'_sum : forall  (l: mset T),  eval (sum' i l) ==eval (sum i l) .
+    Proof.
+      intros [[a n] | [a n] l]; destruct n;  simpl; reflexivity.
+    Qed.
 
-       rewrite <- eval_sum_cons. setoid_rewrite eval_sum_cons at 3. 
-       rewrite plus_com, <- plus_assoc. rewrite plus_com in IHk. rewrite <- IHk.
-       rewrite eval_sum_cons. apply plus_compat; reflexivity. 
-  Qed.
+    Lemma eval_sum_nil x:
+      eval (sum i (nil (x,xH))) == (eval x).
+    Proof. rewrite <- sum'_sum. reflexivity.   Qed.
+     
+    Lemma eval_sum_cons : forall n a (l: mset T),
+      (eval (sum i ((a,n)::l))) == (@Bin.value _ _ (e_bin i) (@copy _ (@Bin.value _ _ (e_bin i)) n (eval a)) (eval (sum i l))).
+    Proof.
+      intros n a [[? ? ]|[b m] l]; simpl; reflexivity.
+    Qed.
+   
+    Inductive compat_sum_unit : @m idx (mset T) -> Prop :=
+    | csu_left : forall x,  is_unit x = true->  compat_sum_unit  (left x)
+    | csu_right : forall m, compat_sum_unit (right m)
+    .
 
-  Inductive sum_spec: T -> option (mset T) -> Prop :=
-  | ss_sum1: forall i l, sum_spec (sum i l) (Some l)
-  | ss_sum2: forall j i l, i<>j -> sum_spec (sum i l) None
-  | ss_prd: forall i l, sum_spec (prd i l) None
-  | ss_sym: forall i l, sum_spec (@sym i l) None.
-  Lemma is_sum_spec: forall i (a: T), sum_spec a (is_sum i a).
-  Proof.
-    intros i [j l|j l|j l]; simpl; try constructor.
-    case eq_idx_spec; intro.
-     subst. constructor.
-     econstructor. eassumption.
-  Qed.
+    Lemma compat_sum_unit_return x n : compat_sum_unit  (return_sum i is_unit x n).
+    Proof.
+      unfold return_sum.
+      case is_sum_spec; intros; try constructor; auto.
+    Qed.
+   
+    Lemma compat_sum_unit_add : forall x n h,
+      compat_sum_unit  h
+      ->
+     compat_sum_unit
+     (add_to_sum i (is_unit_of i) x n
+       h).
+    Proof.
+      unfold add_to_sum;intros; inversion H;
+        case_eq  (is_sum i (is_unit_of i) x);
+        intros; simpl; try constructor || eauto. apply H0.
+    Qed.
 
-  Lemma eval_is_sum: forall i (a: T) k, is_sum i a = Some k -> eval (sum i k) = eval a.
-  Proof.
-    intros i [j l|j l|j l] k; simpl is_sum; try (intro; discriminate).
-    case eq_idx_spec; intros ? H. 
-     injection H. clear H. intros <-. congruence. 
-     discriminate.
-  Qed.
+    (* Hint Resolve copy_plus. : this lags because of  the inference of the implicit arguments *)
+    Hint Extern 5 (copy (?n + ?m) (eval ?a) == Bin.value (copy ?n (eval ?a)) (copy ?m (eval ?a))) => apply copy_plus.
+    Hint Extern 5 (?x == ?x) => reflexivity.
+    Hint Extern 5 ( Bin.value ?x ?y == Bin.value ?y ?x) => apply Bin.comm.
+   
+    Lemma eval_merge_bin : forall (h k: mset T),
+      eval (sum i (merge_msets compare h k)) == @Bin.value _ _ (e_bin i) (eval (sum i h)) (eval (sum i k)).
+    Proof.
+      induction h as [[a n]|[a n] h IHh]; intro k.
+      simpl.
+      induction k as [[b m]|[b m] k IHk]; simpl.
+      destruct (tcompare_weak_spec a b) as [a|a b|a b]; simpl; auto. apply copy_plus; auto.
+     
+      destruct (tcompare_weak_spec a b) as [a|a b|a b]; simpl; auto.
+      rewrite copy_plus,law_assoc; auto. 
+      rewrite IHk;  clear IHk. rewrite 2 law_assoc. apply proper. apply law_comm. reflexivity.
+     
+      induction k as [[b m]|[b m] k IHk]; simpl;  simpl in IHh.
+      destruct (tcompare_weak_spec a b) as [a|a b|a b]; simpl.
+      rewrite  (law_comm _ (copy m (eval a))), law_assoc, <- copy_plus,  Pplus_comm; auto. 
+      rewrite <- law_assoc, IHh.  reflexivity.
+      rewrite law_comm. reflexivity.
+     
+      simpl in IHk.
+      destruct (tcompare_weak_spec a b) as [a|a b|a b]; simpl.
+      rewrite IHh; clear IHh. rewrite 2 law_assoc. rewrite (law_comm _ (copy m (eval a))). rewrite law_assoc, <- copy_plus,  Pplus_comm; auto. 
+      rewrite IHh; clear IHh. simpl.  rewrite law_assoc. reflexivity. 
+      rewrite 2 (law_comm  (copy m (eval b))). rewrite law_assoc.  apply proper; [ | reflexivity]. 
+      rewrite <- IHk. reflexivity.
+    Qed.
 
-  Lemma copy_mset' n (l: mset T): 
-    copy_mset n l = List.map (fun vm => let '(v,m):=vm in (v,Pmult n m)) l.
-  Proof.
-    intros. destruct n; try reflexivity.
-    simpl. induction l as [|[a l] IHl]; simpl; congruence. 
-  Qed.
+ 
+    Lemma copy_mset' n (l: mset T):  copy_mset n l = nelist_map (fun vm => let '(v,m):=vm in (v,Pmult n m)) l.
+    Proof.
+      unfold copy_mset.  destruct n; try reflexivity.
+     
+      simpl. induction l as [|[a l] IHl]; simpl; try congruence.  destruct a.  reflexivity.
+    Qed.
+   
+   
+    Lemma copy_mset_succ  n (l: mset T):  eval (sum i (copy_mset (Psucc n) l)) == @Bin.value _ _ (e_bin i) (eval (sum i l)) (eval (sum i (copy_mset n l))).
+    Proof.
+      rewrite 2 copy_mset'.
+     
+      induction l as [[a m]|[a m] l IHl].
+      simpl eval.   rewrite <- copy_plus; auto. rewrite Pmult_Sn_m. reflexivity.
+     
+      simpl nelist_map.  rewrite ! eval_sum_cons. rewrite IHl.  clear IHl.
+      rewrite Pmult_Sn_m. rewrite copy_plus; auto. rewrite <- !law_assoc.
+      apply Binvalue_Proper; try reflexivity.
+      rewrite law_comm . rewrite <- !law_assoc. apply proper; try reflexivity.
+      apply law_comm.
+    Qed.
 
+    Lemma copy_mset_copy : forall n  (m : mset T), eval (sum i (copy_mset n m)) == @copy _ (@Bin.value _ _ (e_bin i)) n (eval (sum i m)).
+    Proof.
+      induction n using Pind; intros.
+     
+      unfold copy_mset. rewrite copy_xH. reflexivity.
+      rewrite copy_mset_succ. rewrite copy_Psucc. rewrite IHn. reflexivity.
+    Qed.
+   
+    Instance compat_sum_unit_Unit : forall p, compat_sum_unit (left p) ->
+      @Unit X R (Bin.value (e_bin i)) (eval (unit p)).
+    Proof.
+      intros.
+      inversion H. subst.  auto.
+    Qed.
   
-  Lemma copy_mset_succ i n (l: mset T): 
-    eval (sum i (copy_mset (Psucc n) l)) == @Sum.plus _ _ (e_sum i) (eval (sum i l)) (eval (sum i (copy_mset n l))).
+    Lemma copy_n_unit : forall j n, is_unit j = true ->
+      eval (unit j) == @copy _ (Bin.value (e_bin i)) n (eval (unit j)).
+    Proof.
+      intros.
+      induction n using Prect.
+      rewrite copy_xH. reflexivity.
+      rewrite copy_Psucc. rewrite <- IHn. apply is_unit_sum_Unit in H. rewrite law_neutral_left. reflexivity.
+    Qed.
+
+   
+    Lemma z0  l r (H : compat_sum_unit  r):
+      eval (sum i (run_msets (comp (merge_msets compare) l r))) == eval (sum i ((merge_msets compare) (l) (run_msets r))).
+    Proof.
+      unfold comp. unfold run_msets.
+      case_eq r; intros; subst.
+      rewrite eval_merge_bin; auto.
+      rewrite eval_sum_nil.
+      apply compat_sum_unit_Unit in H. rewrite law_neutral_right.  reflexivity.
+      reflexivity.
+    Qed.
+
+    Lemma z1 : forall n x,
+      eval (sum i (run_msets (return_sum i (is_unit) x n )))
+      == @copy _ (@Bin.value _ _ (e_bin i)) n (eval x).
+    Proof.
+      intros. unfold return_sum.  unfold run_msets.
+      case (is_sum_spec); intros; subst.
+      rewrite copy_mset_copy.
+      reflexivity.
+     
+      rewrite eval_sum_nil. apply copy_n_unit. auto.
+      reflexivity.
+    Qed.
+    Lemma z2 : forall  u n x, compat_sum_unit  x ->
+      eval (sum i ( run_msets
+        (add_to_sum i (is_unit) u n x)))
+      == 
+      @Bin.value _ _ (e_bin i) (@copy _ (@Bin.value _ _ (e_bin i))  n (eval u)) (eval (sum i (run_msets x))).
+    Proof.
+      intros u n x Hix .
+      unfold add_to_sum.
+      case is_sum_spec; intros; subst.
+   
+      rewrite z0 by auto.  rewrite eval_merge_bin.  rewrite copy_mset_copy. reflexivity.
+      rewrite <- copy_n_unit by assumption.
+      apply is_unit_sum_Unit in H.
+      rewrite law_neutral_left. reflexivity.
+     
+     
+      rewrite z0 by auto.  rewrite eval_merge_bin. reflexivity.
+    Qed.
+  End sum_correctness.
+  Lemma eval_norm_msets i norm
+    (Comm : Commutative R (Bin.value (e_bin i)))
+    (Hnorm: forall u, eval (norm u) == eval u) : forall h, eval (sum i (norm_msets norm i h)) == eval (sum i h).
   Proof.
-    intros. rewrite 2copy_mset'.
-    induction l as [|[a m] l IHl].
-     simpl eval at 2. rewrite plus_neutral_left. destruct n; reflexivity.
-     simpl map. rewrite ! eval_sum_cons. rewrite IHl. 
-     rewrite Pmult_Sn_m. rewrite copy_plus. rewrite <- !plus_assoc. apply plus_compat; try reflexivity.
-     setoid_rewrite plus_com at 3. rewrite <- !plus_assoc. apply plus_compat; try reflexivity. apply plus_com. 
-  Qed.
-
-  Lemma eval_sum_to_mset: forall i n a, eval (sum i (sum_to_mset i a n)) == @copy _  (@Sum.plus _ _ (e_sum i)) n (eval a).
-  Proof.
-    intros. unfold sum_to_mset.
-    case_eq (is_sum i a).
-     intros k Hk. induction n using Pind. 
-       simpl copy_mset. rewrite (eval_is_sum _ _ Hk). reflexivity.
-       rewrite copy_mset_succ. rewrite IHn. rewrite (eval_is_sum _ _ Hk).
-       unfold copy at 2. rewrite Prect_succ. reflexivity.
-     reflexivity.
-  Qed.
-
-
+    unfold norm_msets.
+    assert (H :
+      forall h : mset T,
+        eval (sum i (run_msets (norm_msets_ i (is_unit_of i) norm h))) ==  eval (sum i h) /\ compat_sum_unit (is_unit_of i) (norm_msets_ i (is_unit_of i) norm h)).
+      
+    induction h as [[a n] | [a n] h [IHh IHh']]; simpl norm_msets_; split.
+    rewrite z1 by auto. rewrite Hnorm . reflexivity. auto.
+    apply compat_sum_unit_return.
+      
+    rewrite z2 by auto. rewrite IHh. 
+    rewrite eval_sum_cons.  rewrite Hnorm. reflexivity. apply compat_sum_unit_add, IHh'.
+   
+    apply H.
+  Defined.
+ 
   (** auxiliary lemmas about products  *)
-  Lemma prd'_prd i (l: list T): eval (prd' i l) == eval (prd i l).
-  Proof. intros i [|? [|? ?]]; reflexivity. Qed.
 
-  Lemma eval_prd_cons i a (l: list T): eval (prd i (a::l)) == @Prd.dot _ _ (e_prd i) (eval a) (eval (prd i l)).
+  Section prd_correctness.
+    Variable i : idx.
+    Variable is_unit : idx -> bool.
+    Hypothesis is_unit_prd_Unit : forall j, is_unit j = true->  @Unit X R (Bin.value (e_bin i)) (eval (unit j)).
+
+    Inductive is_prd_spec_ind  : T ->  @discr (nelist T) -> Prop :=
+    | is_prd_spec_op :
+      forall j l, j = i -> is_prd_spec_ind (prd j l) (Is_op l)
+    | is_prd_spec_unit :
+      forall j, is_unit j = true ->  is_prd_spec_ind (unit j) (Is_unit j)
+    | is_prd_spec_nothing :
+      forall u, is_prd_spec_ind u (Is_nothing).
+   
+    Lemma is_prd_spec u : is_prd_spec_ind u (is_prd i is_unit u).
+    Proof.
+      unfold is_prd; case u; intros; try constructor.
+      case (eq_idx_spec); intros; subst;  try constructor; auto.
+      case_eq (is_unit p); intros; try constructor; auto.  
+    Qed.
+
+    Lemma prd'_prd : forall (l: nelist T), eval (prd' i l) == eval (prd i l).
+    Proof.
+      intros  [?|? [|? ?]]; simpl; reflexivity.
+    Qed.
+   
+   
+    Lemma eval_prd_nil x:  eval (prd i (nil x)) == eval x. 
+    Proof.
+      rewrite <- prd'_prd. simpl. reflexivity.
+    Qed.
+    Lemma eval_prd_cons a : forall (l: nelist T), eval (prd i (a::l)) == @Bin.value _ _ (e_bin i) (eval a) (eval (prd i l)).
+    Proof.
+      intros  [|b l]; simpl; reflexivity.
+    Qed.       
+    Lemma eval_prd_app : forall (h k: nelist T), eval (prd i (h++k)) == @Bin.value _ _ (e_bin i) (eval (prd i h)) (eval (prd i k)).
+    Proof.
+      induction h; intro k. simpl; try reflexivity.
+      simpl appne.  rewrite  2 eval_prd_cons, IHh, law_assoc. reflexivity.
+    Qed.       
+
+    Inductive compat_prd_unit : @m idx (nelist T) -> Prop :=
+    | cpu_left : forall x,  is_unit  x = true -> compat_prd_unit  (left x)
+    | cpu_right : forall m, compat_prd_unit (right m)
+    .
+ 
+    Lemma compat_prd_unit_return  x: compat_prd_unit (return_prd i is_unit x).
+    Proof.
+      unfold return_prd.
+      case (is_prd_spec); intros; try constructor; auto.
+    Qed.
+
+    Lemma compat_prd_unit_add  : forall x  h,
+      compat_prd_unit  h
+      ->
+      compat_prd_unit
+      (add_to_prd i is_unit x
+        h).
+    Proof.
+      intros.
+      unfold add_to_prd.
+      unfold comp.
+      case (is_prd_spec); intros; try constructor; auto.
+      unfold comp; case h; try constructor.
+      unfold comp; case h; try constructor.
+    Qed.
+
+   
+    Instance compat_prd_Unit : forall p, compat_prd_unit (left p) ->
+      @Unit X R (Bin.value (e_bin i)) (eval (unit p)).
+    Proof.
+      intros.
+      inversion H; subst. apply is_unit_prd_Unit. assumption.
+    Qed.
+
+    Lemma z0' : forall l (r: @m idx (nelist T)), compat_prd_unit r ->
+      eval (prd i (run_list (comp (@appne T) l r))) == eval (prd i ((appne (l) (run_list r)))).
+    Proof.
+      intros.
+      unfold comp. unfold run_list. case_eq r; intros; auto; subst.
+      rewrite eval_prd_app.
+      rewrite eval_prd_nil.
+      apply compat_prd_Unit in H. rewrite law_neutral_right. reflexivity.
+      reflexivity.
+    Qed.
+ 
+    Lemma z1' a :  eval (prd i (run_list (return_prd i is_unit a))) ==  eval (prd i (nil a)).
+    Proof.
+      intros. unfold return_prd.  unfold run_list.
+      case (is_prd_spec); intros; subst; reflexivity.
+    Qed.
+    Lemma z2' : forall  u  x, compat_prd_unit  x -> 
+      eval (prd i ( run_list
+        (add_to_prd i is_unit u x))) ==  @Bin.value _ _ (e_bin i) (eval u) (eval (prd i (run_list x))).
+    Proof.
+      intros u x Hix.
+      unfold add_to_prd.
+      case (is_prd_spec); intros; subst.
+      rewrite z0' by auto.  rewrite eval_prd_app.  reflexivity.
+      apply is_unit_prd_Unit in H. rewrite law_neutral_left. reflexivity.
+      rewrite z0' by auto.  rewrite eval_prd_app. reflexivity.
+    Qed.
+ 
+  End prd_correctness.
+
+
+
+
+  Lemma eval_norm_lists i (Hnorm: forall u, eval (norm u) == eval u) : forall h, eval (prd i (norm_lists norm i h)) == eval (prd i h).
   Proof.
-    intros i a [|b l]; simpl. 
-     rewrite dot_neutral_right. reflexivity.
-     reflexivity.
-  Qed.        
+    unfold norm_lists.
+    assert (H :  forall h : nelist T,
+      eval (prd i (run_list (norm_lists_ i (is_unit_of i) norm h))) ==
+      eval (prd i h)
+      /\ compat_prd_unit (is_unit_of i) (norm_lists_ i (is_unit_of i) norm h)).
+  
+   
+      induction h as [a | a h [IHh IHh']]; simpl norm_lists_; split.
+      rewrite z1'. simpl.  apply Hnorm.
+   
+      apply compat_prd_unit_return.
+   
+      rewrite z2'. rewrite IHh.  rewrite eval_prd_cons.  rewrite Hnorm. reflexivity. apply is_unit_of_Unit.
+      auto.
 
-  Lemma eval_prd_app i (h k: list T): eval (prd i (h++k)) == @Prd.dot _ _ (e_prd i) (eval (prd i h)) (eval (prd i k)).
-  Proof.
-    induction h; intro k. 
-     simpl. rewrite dot_neutral_left. reflexivity.
-     simpl app. rewrite 2 eval_prd_cons, IHh, dot_assoc. reflexivity.
-  Qed.        
-
-  Lemma eval_is_prd: forall i (a: T) k, is_prd i a = Some k -> eval (prd i k) = eval a.
-  Proof.
-    intros i [j l|j l|j l] k; simpl is_prd; try (intro; discriminate).
-    case eq_idx_spec; intros ? H. 
-     injection H. clear H. intros <-. subst. congruence.
-     discriminate.
-  Qed.
-
-  Lemma eval_prd_to_list: forall i a, eval (prd i (prd_to_list i a)) = eval a.
-  Proof.
-    intros. unfold prd_to_list.
-    case_eq (is_prd i a).
-     intros k Hk. apply eval_is_prd. assumption.
-     reflexivity.
-  Qed.
-
+      apply compat_prd_unit_add. auto.
+      apply H.
+    Defined.
 
   (** correctness of the normalisation function *)
+
   Theorem eval_norm: forall u, eval (norm u) == eval u
-    with eval_norm_aux: forall i (l: vT i) (f: Sym.type_of i), 
+    with eval_norm_aux: forall i (l: vT i) (f: Sym.type_of i),
       Proper (@Sym.rel_of X R i) f -> eval_aux (vnorm l) f == eval_aux l f.
   Proof.
-    induction u.
-     simpl norm. rewrite sum'_sum. induction m as [|[u n] m IHm]. 
-      reflexivity.
-      simpl merge_map. rewrite eval_merge_sum.
-      rewrite eval_sum_to_mset, IHm, eval_norm.
-      rewrite eval_sum_cons. reflexivity.
+    induction u as [ p m | p l | ? | ?];  simpl norm.
+    case_eq (is_commutative p); intros.
+    rewrite sum'_sum.
+    apply eval_norm_msets; auto.
+    reflexivity.
 
-     simpl norm. rewrite prd'_prd. induction l. 
-      reflexivity.
-      simpl merge_map.
-      rewrite eval_prd_app.
-      rewrite eval_prd_to_list, IHl, eval_norm.
-      rewrite eval_prd_cons. reflexivity.
+    rewrite prd'_prd.
+    apply eval_norm_lists; auto.
 
-     simpl. apply eval_norm_aux, Sym.morph. 
+    apply eval_norm_aux, Sym.morph.
 
+    reflexivity.
 
-    induction l; simpl; intros f Hf.
-     reflexivity.
-     rewrite eval_norm. apply IHl, Hf. reflexivity.
+    induction l; simpl; intros f Hf. reflexivity.
+    rewrite eval_norm. apply IHl, Hf; reflexivity.
   Qed.
 
+
   (** corollaries, for goal normalisation or decision *)
-  Lemma normalise: forall (u v: T), eval (norm u) == eval (norm v) -> eval u == eval v.
+
+  Lemma normalise : forall (u v: T), eval (norm u) == eval (norm v) -> eval u == eval v.
   Proof. intros u v. rewrite 2 eval_norm. trivial. Qed.
-    
+   
   Lemma compare_reflect_eq: forall u v, compare u v = Eq -> eval u == eval v.
   Proof. intros u v. case (tcompare_weak_spec u v); intros; try congruence. reflexivity. Qed.
 
   Lemma decide: forall (u v: T), compare (norm u) (norm v) = Eq -> eval u == eval v.
   Proof. intros u v H. apply normalise. apply compare_reflect_eq. apply H. Qed.
 
+  Lemma lift_normalise {S} {H : AAC_lift S R}:
+    forall (u v: T), (let x := norm u in let y := norm v in
+      S (eval x) (eval y)) -> S (eval u) (eval v).
+  Proof. destruct H. intros u v; simpl; rewrite 2 eval_norm. trivial. Qed.
+
 End s.
+End Internal.
+
+
+(** * Lemmas for performing transitivity steps
+   given an instance of AAC_lift *)
+
+Section t.
+  Context `{AAC_lift}.
+
+  Lemma lift_transitivity_left  (y x z : X): E x y -> R y z -> R x z.
+  Proof. destruct H as [Hequiv Hproper]; intros G;rewrite G. trivial. Qed.
+ 
+  Lemma lift_transitivity_right (y x z : X): E y z -> R x y -> R x z.
+  Proof.  destruct H as [Hequiv Hproper]; intros G. rewrite G. trivial. Qed.
+
+  Lemma lift_reflexivity {HR :Reflexive R}: forall x y, E x y -> R x y.
+  Proof. destruct H. intros ? ? G. rewrite G. reflexivity. Qed.
+
+End t.
+       
 Declare ML Module "aac_tactics".
