Tutorial.v
@@ -6,97 +6,70 @@
 (*       Copyright 2009-2010: Thomas Braibant, Damien Pous.                *)
 (***************************************************************************)
 
-(** * Examples about uses of the aac_rewrite library *)
+(** * Tutorial for using the [aac_tactics] library.
 
-(*
-   Depending on your installation, either uncomment the following two
-   lines, or add them to your .coqrc files, replacing path_to_aac_tactics
-   with the correct path for your installation:
+   Depending on your installation, either modify the following two
+   lines, or add them to your .coqrc files, replacing "."  with the
+   path to the [aac_tactics] library. *)
 
-   Add Rec LoadPath "path_to_aac_tactics".
-   Add ML Path "path_to_aac_tactics".
-*)
-Require Export  AAC.
+Add Rec LoadPath "." as AAC_tactics.
+Add ML Path ".".
+Require Import AAC.
 Require Instances.
 
-(** ** Introductory examples  *)
+(** ** Introductory example 
 
-(** First, we settle in the context of Z, and show an usage of our
-tactics: we rewrite an universally quantified hypothesis modulo
-associativity and commutativity. *)
+   Here is a first example with relative numbers ([Z]): one can
+   rewrite an universally quantified hypothesis modulo the
+   associativity and commutativity of [Zplus]. *)
 
 Section introduction.
+
   Import ZArith.
   Import Instances.Z.
-  
+
   Variables a b c : Z.
   Hypothesis H: forall x, x + Zopp x = 0.
   Goal a + b + c + Zopp (c + a) = b.
     aac_rewrite H.
     aac_reflexivity.
   Qed.
-  Goal a + c+ Zopp (b + a + Zopp b) = c.
+  Goal a + c + Zopp (b + a + Zopp b) = c.
     do 2 aac_rewrite H.
     reflexivity.
   Qed.
 
-  (** Notes: 
+  (** Notes:
      - the tactic handles arbitrary function symbols like [Zopp] (as
-       long as they are proper morphisms);
+       long as they are proper morphisms w.r.t. the considered
+       equivalence relation);
      - here, ring would have done the job.
      *)
 
-End introduction.  
+End introduction. 
 
-(** Second, we show how to exploit binomial identities to prove a goal
-about pythagorean triples, without breaking a sweat. By comparison,
-even if the goal and the hypothesis are both in normal form, making
-the rewrites using standard tools is difficult.
-*)
 
-Section binomials.
+(** ** Usage
 
-  Import ZArith.
-  Import Instances.Z.
- 
-  Notation "x ^2" := (x*x) (at level 40).
-  Notation "2 ⋅ x" := (x+x) (at level 41).
-  Lemma Hbin1: forall x y, (x+y)^2   = x^2 + y^2 +  2⋅x*y. Proof. intros; ring. Qed.
-  Lemma Hbin2: forall x y, x^2 + y^2 = (x+y)^2   + -(2⋅x*y). Proof. intros; ring.  Qed.
-  Lemma Hopp : forall x, x + -x = 0. Proof Zplus_opp_r.  
-  
-  Variables a b c : Z.
-  Hypothesis H : c^2 + 2⋅(a+1)*b  = (a+1+b)^2.
-  Goal a^2 + b^2 + 2⋅a + 1 = c^2.
-    aacu_rewrite <- Hbin1.
-    aac_rewrite Hbin2.
-    aac_rewrite <- H.
-    aac_rewrite Hopp.
-    aac_reflexivity.
-  Qed.
-
-  (** Note: after the [aac_rewrite <- H], one could use [ring] to close the proof.*)
-
-End binomials.
-
-(** ** Usage *)
-
-(** One can also work in an abstract context, with arbitrary
-   associative and commutative operators.
-
-   (Note that one can declare several operations of each kind;
-   however, to be able to use this plugin, one currently needs at least
-   one associative operator, and one associative-commutative
-   operator.) *)
+   One can also work in an abstract context, with arbitrary
+   associative and commutative operators. (Note that one can declare
+   several operations of each kind.) *)
 
 Section base.
-  
-  Context {X} {R} {E: Equivalence R} 
-  {plus} {zero}
-  {dot} {one}
-  {A:  @Op_A X R dot one}        
-  {AC: Op_AC R plus zero}.      
- 
+  Context {X} {R} {E: Equivalence R}
+  {plus}
+  {dot}
+  {zero}
+  {one}
+  {dot_A:  @Associative X R dot }       
+  {plus_A: @Associative X R plus }
+  {plus_C: @Commutative X R plus }
+  {dot_Proper :Proper (R ==> R ==> R) dot}
+  {plus_Proper :Proper (R ==> R ==> R) plus}
+  {Zero : Unit R plus zero}
+  {One : Unit R dot one}
+  .     
+
   Notation "x == y"  := (R x y) (at level 70).
   Notation "x * y"   := (dot x y) (at level 40, left associativity).
   Notation "1"       := (one).
@@ -110,30 +83,32 @@ Section base.
   Section reminder.
     Hypothesis H : forall x, x * x == x.
     Variables a b c : X.
-    
+   
     Goal (a+b+c)*(c+a+b) == a+b+c.
       aac_rewrite H.
       aac_reflexivity.
     Qed.
 
-    (** Note: the tactic starts by normalizing terms, so that trailing
-    units are always eliminated. *)
+    (** The tactic starts by normalising terms, so that trailing units
+    are always eliminated. *)
 
     Goal ((a+b)+0+c)*((c+a)+b*1) == a+b+c.
       aac_rewrite H.
       aac_reflexivity.
     Qed.
   End reminder.
-  
-  (** We can deal with "proper" morphisms of arbitrary arity (here [f],
-     or [Zopp] earlier), and rewrite under morphisms (here [g]). *)
+ 
+  (** The tactic can deal with "proper" morphisms of arbitrary arity
+     (here [f] and [g], or [Zopp] earlier): it rewrites under such
+     morphisms ([g]), and, more importantly, it is able to reorder
+     terms modulo AC under these morphisms ([f]). *)
 
   Section morphisms.
     Variable f : X -> X -> X.
     Hypothesis Hf : Proper (R ==> R ==> R) f.
     Variable g : X -> X.
     Hypothesis Hg : Proper (R ==> R) g.
-    
+   
     Variable a b: X.
     Hypothesis H : forall x y, x+f (b+y) x == y+x.
     Goal g ((f (a+b) a) + a) == g (a+a).
@@ -142,180 +117,283 @@ Section base.
     Qed.
   End morphisms.
 
-  (** ** Selecting what and where to rewrite  *)
+  (** *** Selecting what and where to rewrite 
 
-  (** There are sometimes several possible rewriting. We now show how
-  to interact with the tactic to select the desired one. *)
+     There are sometimes several solutions to the matching problem. We
+     now show how to interact with the tactic to select the desired
+     one. *)
 
   Section occurrence.
-    Variable f : X -> X  .
+    Variable f : X -> X.
     Variable a : X.
     Hypothesis Hf : Proper (R ==> R) f.
-    Hypothesis H : forall x, x + x == x. 
+    Hypothesis H : forall x, x + x == x.
 
     Goal f(a+a)+f(a+a) == f a.
       (** In case there are several possible solutions, one can print
          the different solutions using the [aac_instances] tactic (in
-         proofgeneral, look at buffer *coq* ): *)
+         proof-general, look at buffer *coq* ): *)
       aac_instances H.
-      (** the default choice is the smallest possible context (number
-      0), but one can choose the desired context; *)
-      aac_rewrite H subterm 1.            
-      (** now the goal is [f a + f a  == f a], there is only one solution. *)      
+      (** the default choice is the occurrence with the smallest
+      possible context (number 0), but one can choose the desired
+      one; *)
+      aac_rewrite H at 1.           
+      (** now the goal is [f a + f a  == f a], there is only one solution. *)     
       aac_rewrite H.
       reflexivity.
     Qed.
-  
+ 
   End occurrence.
 
   Section subst.
     Variables a b c d : X.
     Hypothesis H: forall x y, a*x*y*b == a*(x+y)*b.
     Hypothesis H': forall x, x + x == x.
-    
+   
     Goal a*c*d*c*d*b  == a*c*d*b.
-    (** Here, there is only one possible context, but several substitutions; *)
+    (** Here, there is only one possible occurrence, but several substitutions; *)
       aac_instances H.
-      (** we can select them with the proper keyword.  *)
-      aac_rewrite H subst 1. 
+      (** one can select them with the proper keyword.  *)
+      aac_rewrite H subst 1.
       aac_rewrite H'.
       aac_reflexivity.
     Qed.
   End subst.
-  
-  (** As expected, one can use both keyword together to select the
-     correct subterm and the correct substitution. *)
+ 
+  (** As expected, one can use both keywords together to select the
+     occurrence and the substitution. We also provide a keyword to
+     specify that the rewrite should be done in the right-hand side of
+     the equation. *)
 
   Section both.
     Variables a b c d : X.
     Hypothesis H: forall x y, a*x*y*b == a*(x+y)*b.
     Hypothesis H': forall x, x + x == x.
-    
-    Goal a*c*d*c*d*b*b == a*(c*d+b)*b.
+   
+    Goal a*c*d*c*d*b*b == a*(c*d*b)*b.
       aac_instances H.
-      aac_rewrite H subterm 1 subst 1.
+      aac_rewrite H at 1 subst 1.
+      aac_instances H.
       aac_rewrite H.
       aac_rewrite H'.
+      aac_rewrite H at 0 subst 1 in_right.
       aac_reflexivity.
     Qed.
-      
+     
   End both.
 
-  (** We now turn on explaining the distinction between [aac_rewrite]
-  and [aacu_rewrite]: [aac_rewrite] rejects solutions in which
-  variables are instantiated by units, the companion tactic,
-  [aacu_rewrite] allows such solutions.  *)
+  (** *** Distinction between [aac_rewrite] and [aacu_rewrite]:
+
+  [aac_rewrite] rejects solutions in which variables are instantiated
+  by units, while the companion tactic, [aacu_rewrite] allows such
+  solutions.  *)
 
   Section dealing_with_units.
     Variables a b c: X.
     Hypothesis H: forall x, a*x*a == x.
     Goal a*a == 1.
-      (** Here, x must be instantiated with 1, hence no solutions; *)
-      aac_instances H.            
-      (** while we get solutions with the "aacu" tactic. *)      
+      (** Here, [x] must be instantiated with [1], so that the [aac_*]
+         tactics give no solutions; *)
+      try aac_instances H.           
+      (** while we get solutions with the [aacu_*] tactics. *)     
       aacu_instances H.
       aacu_rewrite H.
       reflexivity.
     Qed.
-      
+     
     (** We introduced this distinction because it allows us to rule
     out dummy cases in common situations: *)
 
     Hypothesis H': forall x y z,  x*y + x*z == x*(y+z).
-    Goal a*b*c + a*c+ a*b == a*(c+b*(1+c)).
+    Goal a*b*c + a*c + a*b == a*(c+b*(1+c)).
     (** 6 solutions without units,  *)
-      aac_instances H'.
+      aac_instances H'.        
+      aac_rewrite H' at 0.
     (** more than 52 with units. *)
       aacu_instances H'.
-    Abort.    
-    
-  End dealing_with_units.  
+    Abort.
+
+  End dealing_with_units. 
 End base.
 
-(** ** Declaring instances *)
+(** *** Declaring instances
 
-(** One can use one's own operations: it suffices to declare them as
-   instances of our classes. (Note that these instances are already
-   declared in file [Instances.v].) *)
+   To use one's own operations: it suffices to declare them as
+   instances of our classes. (Note that the following instances are
+   already declared in file [Instances.v].) *)
 
 Section Peano.
   Require Import Arith.
-     
-  Program  Instance nat_plus : Op_AC eq plus O.
-  Solve All Obligations using firstorder.
+    
+  Instance aac_plus_Assoc : Associative eq plus := plus_assoc.
+  Instance aac_plus_Comm : Commutative eq plus :=  plus_comm.
+ 
+  Instance aac_one : Unit eq mult 1 :=
+    Build_Unit eq mult 1 mult_1_l mult_1_r. 
+  Instance aac_zero_plus : Unit eq plus O :=
+    Build_Unit eq plus (O) plus_0_l plus_0_r.
+ 
 
-  Program  Instance nat_dot : Op_AC eq mult 1.
-  Solve All Obligations using firstorder.
-  
+  (** Two (or more) operations may share the same units: in the
+  following example, [0] is understood as the unit of [max] as well as
+  the unit of [plus]. *)
 
-  (** Caveat: we need at least an instance of an operator that is AC
-   and one that is A for a given relation. However, one can reuse an
-   AC operator as an A operator. *)
+  Instance aac_max_Comm : Commutative eq Max.max :=  Max.max_comm.
+  Instance aac_max_Assoc : Associative eq Max.max := Max.max_assoc.
 
-  Definition default_a := AC_A nat_dot. Existing Instance default_a.
-End Peano.
+  Instance aac_zero_max : Unit eq Max.max  O :=
+    Build_Unit eq Max.max 0 Max.max_0_l Max.max_0_r. 
 
-(** ** Caveats  *)
+  Variable a b c : nat.
+  Goal Max.max (a + 0) 0 = a.
+    aac_reflexivity.
+  Qed.
+   
+  (** Furthermore, several operators can be mixed: *)
 
-Section Peano'.
-  Import Instances.Peano.
-
-  (** 1. We have a special treatment for units, thus, [S x + x] does not
-    match [S 0], which is considered as a unit (one) of the mult
-    operation. *)
-
-  Section caveat_one.
-    Definition double_plus_one x := 2*x + 1. 
-    Hypothesis H : forall x, S x + x = double_plus_one x.
-    Goal S O = double_plus_one O.
-      try aac_rewrite H.         (** 0 solutions (normal since it would use 0 to instantiate x) *)
-      try aacu_rewrite H.        (** 0 solutions (abnormal) *)
-    Abort.
-  End caveat_one.
-
-  (** 2. We cannot at the moment have two classes with the same
-  units: in the following example, [0] is understood as the unit of
-  [max] rather than as the unit of [plus]. *)
-
-  Section max.
-    Program Instance aac_max  : Op_AC eq Max.max O  := Build_Op_AC _ _ _ Max.max_assoc Max.max_comm.
-    Variable a : nat.
-    Goal 0 +  a = a.
-      try aac_reflexivity.
-    Abort.
-  End max.
-End Peano'.
-
-(** 3. If some computations are possible in the goal or in the
-hypothesis, the inference mechanism we use will make the
-conversion. However, it seems that in most cases, these conversions
-can be done by hand using simpl rather than rewrite. *)
-
-Section Z.
-
-  (* The order of the following lines is important in order to get the right scope afterwards. *)
-  Import ZArith.
-  Open Scope Z_scope.
-  Opaque Zmult.
-  
-  Hypothesis dot_ann_left :forall x, x * 0 = 0. 
-  Hypothesis dot_ann_right :forall x, 0 * x = 0. 
-
-  Goal forall a, a*0 = 0.
-    intros. aacu_rewrite dot_ann_left. reflexivity.
+  Hypothesis H : forall x y z, Max.max (x + y) (x + z) = x+ Max.max y z.
+ 
+  Goal Max.max (a + b) (c + (a * 1)) = Max.max c b + a.
+    aac_instances H. aac_rewrite H. aac_reflexivity.
+  Qed. 
+  Goal Max.max (a + b) (c + Max.max (a*1+0) 0) = a + Max.max b c.
+    aac_instances H. aac_rewrite H. aac_reflexivity.
   Qed.
 
-  (** Here the tactic fails, since the 0*a is converted to 0, and no
-  rewrite can occur (even though Zmult is opaque). *)
-  Goal forall a,  0*a = 0.
-    intros. try aacu_rewrite dot_ann_left.
-  Abort. 
-
-  (**  Here the tactic fails, since the 0*x is converted to 0 in the hypothesis. *)
-  Goal forall a,  a*0 = 0.
-    intros. try aacu_rewrite dot_ann_right.
-  Abort. 
-  
  
-End Z.
+  (** *** Working with inequations
+
+     To be able to use the tactics, the goal must be a relation [R]
+     applied to two arguments, and the rewritten hypothesis must end
+     with a relation [Q] applied to two arguments. These relations are
+     not necessarily equivalences, but they should be related
+     according to the occurrence where the rewrite takes place; we
+     leave this check to the underlying call to [setoid_rewrite].  *)
+
+  (** One can rewrite equations in the left member of inequations, *)
+  Goal (forall x, x + x = x) -> a + b + b + a <= a + b.
+    intro Hx.
+    aac_rewrite Hx.
+    reflexivity.
+  Qed.
+
+  (** or in the right member of inequations, using the [in_right] keyword  *)
+  Goal (forall x, x + x = x) -> a + b  <= a + b + b + a.
+    intro Hx.
+    aac_rewrite Hx in_right.
+    reflexivity.
+  Qed.
+ 
+  (** Similarly, one can rewrite inequations in inequations, *)
+  Goal (forall x, x + x <= x) -> a + b + b + a <= a + b.
+    intro Hx.
+    aac_rewrite Hx.
+    reflexivity.
+  Qed. 
+
+  (** possibly in the right-hand side. *)
+  Goal (forall x, x <= x + x) -> a + b <= a + b + b + a.
+    intro Hx.
+    aac_rewrite <- Hx in_right.
+    reflexivity.
+  Qed.
+
+  (** [aac_reflexivity] deals with "trivial" inequations too *)
+  Goal Max.max (a + b) (c + a) <= Max.max (b + a) (c + 1*a).
+    aac_reflexivity.
+  Qed.
+
+  (** In the last three examples, there were no equivalence relation
+     involved in the goal. However, we actually had to guess the
+     equivalence relation with respect to which the operators
+     ([plus,max,0]) were AC.  In this case, it was Leibniz equality
+     [eq] so that it was automatically inferred; more generally, one
+     can specify which equivalence relation to use by declaring
+     instances of the [AAC_lift] type class: *)
+
+  Instance lift_le_eq : AAC_lift le eq.
+  (** (This instance is automatically inferred because [eq] is always a
+     valid candidate, here for [le].) *)
+
+
+End Peano.
+
+
+(** *** Normalising goals
+
+   We also provide a tactic to normalise terms modulo AC. This
+   normalisation is the one we use internally.  *)
+
+Section AAC_normalise.
+
+  Import Instances.Z.
+  Require Import ZArith.
+  Open Scope Z_scope.
+ 
+  Variable a b c d : Z.
+  Goal a + (b + c*c*d) + a + 0 + d*1 = a.
+    aac_normalise.
+  Abort.
+
+End AAC_normalise.
+
+
+
+
+(** ** Examples from the web page *)
+Section Examples.
+
+  Import Instances.Z.
+  Require Import ZArith.
+  Open Scope Z_scope.
+
+  (** *** Reverse triangle inequality *)
+
+  Lemma Zabs_triangle : forall x y,  Zabs (x + y) <= Zabs x + Zabs y .
+  Proof Zabs_triangle.
+
+  Lemma Zplus_opp_r : forall x, x + -x = 0.
+  Proof Zplus_opp_r.
+
+  (** The following morphisms are required to perform the required rewrites *)
+  Instance Zminus_compat : Proper (Zge ==> Zle) Zopp.
+  Proof. intros x y. omega. Qed.
+ 
+  Instance Proper_Zplus : Proper (Zle ==> Zle ==> Zle) Zplus.
+  Proof. firstorder. Qed.
+
+  Goal forall a b, Zabs a - Zabs b <= Zabs (a - b).
+    intros. unfold Zminus.
+    aac_instances <- (Zminus_diag b).
+    aac_rewrite <- (Zminus_diag b) at 3.
+    unfold Zminus.
+    aac_rewrite Zabs_triangle.
+    aac_rewrite Zplus_opp_r.
+    aac_reflexivity.
+  Qed.
+
+
+  (** *** Pythagorean triples *)
+
+  Notation "x ^2" := (x*x) (at level 40).
+  Notation "2 ⋅ x" := (x+x) (at level 41).
+
+  Lemma Hbin1: forall x y, (x+y)^2   = x^2 + y^2 +  2⋅x*y. Proof. intros; ring. Qed.
+  Lemma Hbin2: forall x y, x^2 + y^2 = (x+y)^2   + -(2⋅x*y). Proof. intros; ring.  Qed.
+  Lemma Hopp : forall x, x + -x = 0. Proof Zplus_opp_r. 
+ 
+  Variables a b c : Z.
+  Hypothesis H : c^2 + 2⋅(a+1)*b  = (a+1+b)^2.
+  Goal a^2 + b^2 + 2⋅a + 1 = c^2.
+    aacu_rewrite <- Hbin1.
+    rewrite Hbin2.
+    aac_rewrite <- H.
+    aac_rewrite Hopp.
+    aac_reflexivity.
+  Qed.
+
+  (** Note: after the [aac_rewrite <- H], one could use [ring] to close the proof.*)
+
+End Examples.
+
 
